preimage finished, second preimage to finish to debug, and collision to CC from preimage

sha3/proof/SHA3OSecurity.ec
@@ -5,6 +5,8 @@ require import Common SLCommon Sponge SHA3_OIndiff.
 require (****) SecureORO SecureHash.
 (*****) import OIndif.
 
+require import PROM.
+
 
 (* module SHA3 (P : DPRIMITIVE) = { *)
 (*   proc init() : unit = {} *)
@@ -171,14 +173,25 @@ module FIgnoreSize (F : OIndif.ODFUNCTIONALITY) : OFUNCTIONALITY = {
 module (OSponge : OIndif.OCONSTRUCTION) (P : OIndif.ODPRIMITIVE) = 
   FSetSize(CSome(Sponge,P)).
 
+
+clone import Program as PBool with
+  type t <- bool,
+  op d <- dbool
+proof *.
+
+clone import GenEager as Eager with
+  type from <- bool list * int,
+  type to <- bool,
+  op sampleto <- fun _ => dbool
+proof * by smt(dbool_ll).
+
 section Preimage.
-(* TODO : stopped here *)
 
   declare module A : SH.AdvPreimage { Perm, Counter, Bounder, F.RO, F.FRO, 
     Redo, C, Gconcl.S, BlockSponge.BIRO.IRO, BlockSponge.C, BIRO.IRO, 
     Gconcl_list.BIRO2.IRO, Gconcl_list.F2.RO, Gconcl_list.F2.FRO, 
     Gconcl_list.Simulator, SHA3Indiff.Simulator, SHA3Indiff.Cntr, 
-    SORO.Bounder, RO.RO }.
+    SORO.Bounder, SORO.RO.RO, RO, FRO }.
 
   local module FInit (F : OIndif.ODFUNCTIONALITY) : OIndif.OFUNCTIONALITY = {
     proc init () = {}
@@ -203,16 +216,13 @@ local module Log = {
 
 local module ExtendOutputSize (F : Oracle) : ODFUNCTIONALITY = {
   proc f (x : bool list, k : int) = {
-    var o, l, prefix, suffix, i;
+    var o, l, suffix, prefix, i;
     l <- None;
-    i <- 0;
     prefix <- [];
     suffix <- [];
     o <@ F.get(x);
-    if (o <> None) {
-      prefix <- take k (to_list (oget o));
-      i <- size_out;
-    }
+    prefix <- take k (to_list (oget o));
+    i <- size_out;
     while (i < k) {
       if ((x,i) \notin Log.m) {
         Log.m.[(x,i)] <$ {0,1};
@@ -296,16 +306,6 @@ local module RFWhile = {
   proc sample (x: bool list) = {}
 }.
 
-module type TOTO (F : Oracle) = {
-  proc main () : bool
-}.
-
-clone import Program as PBool with
-  type t <- bool,
-  op d <- dbool
-proof *.
-
-
 local equiv rw_RF_List_While :
     RFList.get ~ RFWhile.get : 
     ={arg, glob RFList} ==> ={res, glob RFWhile}.
@@ -339,7 +339,7 @@ local equiv eq_IRO_RFWhile :
   BIRO.IRO.f ~ RFWhile.get :
   arg{1} = (x{2}, size_out) /\ inv BIRO.IRO.mp{1} RFList.m{2}
   ==>
-  res{2} = of_list res{1} /\ inv BIRO.IRO.mp{1} RFList.m{2}.
+  res{2} = of_list res{1} /\ size res{1} = size_out /\ inv BIRO.IRO.mp{1} RFList.m{2}.
 proof.
 proc; inline*; sp.
 rcondt{1} 1; 1: by auto.
@@ -405,21 +405,247 @@ while(l{2} = bs{1} /\ size bs{1} = i{1} /\ 0 <= i{1} <= n{1} /\ ={i} /\
 by auto; smt(size_out_gt0).
 qed.
 
+
 op eq_extend_size (m1 : (bool list * int, bool) fmap) (m2 : (bool list * int, bool) fmap)
   (m3 : (bool list * int, bool) fmap) =
+  (* (forall x j, (x,j) \in m2 => 0 <= j < size_out) /\ *)
+  (* (forall x j, (x,j) \in m2 => forall k, 0 <= k < size_out => (x, k) \in m2) /\ *)  
   (forall x j, 0 <= j < size_out => m1.[(x,j)] = m2.[(x,j)]) /\
   (forall x j, size_out <= j => m1.[(x,j)] = m3.[(x,j)]) /\
   (forall x j, (x,j) \in m1 => 0 <= j).
 
+local module ExtendSample (F : OFUNCTIONALITY) = {
+  proc init = F.init
+  proc f (x : bool list, k : int) = {
+    var y;
+    if (k <= size_out) {
+      y <@ F.f(x,size_out);
+      y <- omap (take k) y;
+    } else {
+      y <@ F.f(x,k);
+    }
+    return y;
+  }
+}.
+
 
 local equiv eq_extend :
-  FSome(BIRO.IRO).f ~ ExtendOutputSize(FSetSize(FSome(BIRO.IRO))).f :
+  ExtendSample(FSome(BIRO.IRO)).f ~ ExtendOutputSize(FSetSize(FSome(BIRO.IRO))).f :
   ={arg} /\ eq_extend_size BIRO.IRO.mp{1} BIRO.IRO.mp{2} Log.m{2} ==>
   ={res} /\ eq_extend_size BIRO.IRO.mp{1} BIRO.IRO.mp{2} Log.m{2}.
 proof.
 proc; inline*; auto; sp.
-rcondt{1} 1; auto; rcondt{2} 1; auto.
+rcondt{2} 1; 1: auto.
+if{1}; sp.
+- rcondt{1} 1; auto.
+  rcondf{2} 8; 1: auto.
+  - conseq(:_==> true); 1: smt(). 
+    by while(true); auto.
+  auto=> /=.
+  conseq(:_==> ={bs, k} /\ size bs{1} = size_out /\
+    eq_extend_size BIRO.IRO.mp{1} BIRO.IRO.mp{2} Log.m{2})=> //=.
+  - smt(cats0 to_listK spec2_dout).
+  while(={k, bs, n, x2} /\ i{1} = i0{2} /\ n{1} = size_out /\
+      0 <= i{1} <= n{1} /\ size bs{1} = i{1} /\
+      eq_extend_size BIRO.IRO.mp{1} BIRO.IRO.mp{2} Log.m{2}).
+  - by sp; if; auto; smt(domE get_setE size_rcons).
+  by auto; smt(size_eq0 size_out_gt0).
+rcondt{1} 1; 1: auto.
+splitwhile{1} 1 : i0 < size_out; auto=> /=.
+while( (i0, n0, x3){1} = (i, k, x){2} /\ bs0{1} = prefix{2} ++ suffix{2} /\
+    size_out <= i{2} <= k{2} /\ eq_extend_size BIRO.IRO.mp{1} BIRO.IRO.mp{2} Log.m{2}).
++ by sp; if; auto; smt(domE get_setE size_out_gt0 rcons_cat).
+auto=> //=.
+conseq(:_==> ={i0} /\ size bs{2} = i0{1} /\ (i0, x3){1} = (n, x2){2} /\
+    bs0{1} = bs{2} /\ size bs{2} = size_out /\
+    eq_extend_size BIRO.IRO.mp{1} BIRO.IRO.mp{2} Log.m{2}). 
++ smt(cats0 take_oversize spec_dout to_listK spec2_dout).
+while(={i0} /\ x3{1} = x2{2} /\ 0 <= i0{1} <= n{2} /\ n{2} = size_out /\
+    bs0{1} = bs{2} /\ size bs{2} = i0{1} /\ size_out <= n0{1} /\
+    eq_extend_size BIRO.IRO.mp{1} BIRO.IRO.mp{2} Log.m{2}).
++ by sp; if; auto; smt(size_rcons domE get_setE size_rcons mem_set).
+by auto; smt(size_out_gt0).
 qed.
+
+
+local lemma of_listK l : of_list (to_list l) = Some l.
+proof.
+by rewrite -to_listK.
+qed.
+
+local module Fill_In (F : RO) = {
+  proc init = F.init
+  proc f (x : bool list, n : int) = {
+    var l, b, i;
+    i <- 0;
+    l <- [];
+    while (i < n) {
+      b <@ F.get((x,i));
+      l <- rcons l b;
+      i <- i + 1;
+    }
+    while (i < size_out) {
+      F.sample((x,i));
+      i <- i + 1;
+    }
+    return l;
+  }
+}.
+
+print module RO.
+
+local equiv eq_eager_ideal :
+  BIRO.IRO.f ~ Fill_In(LRO).f :
+  ={arg} /\ BIRO.IRO.mp{1} = RO.m{2} ==>
+  ={res} /\ BIRO.IRO.mp{1} = RO.m{2}.
+proof.
+proc; inline*; sp; rcondt{1} 1; auto.
+while{2}(bs{1} = l{2} /\ BIRO.IRO.mp{1} = RO.m{2})(size_out - i{2}).
++ by auto=> />; smt().
+conseq(:_==> bs{1} = l{2} /\ BIRO.IRO.mp{1} = RO.m{2}); 1: smt().
+while(={i, n, x} /\ bs{1} = l{2} /\ BIRO.IRO.mp{1} = RO.m{2}).
++ sp; if{1}.
+  - by rcondt{2} 2; auto=> />.
+  by rcondf{2} 2; auto=> />; smt(dbool_ll).
+by auto.
+qed.
+
+local equiv eq_eager_ideal2 :
+  ExtendSample(FSome(BIRO.IRO)).f ~ FSome(Fill_In(RO)).f :
+  ={arg} /\ BIRO.IRO.mp{1} = RO.m{2} ==>
+  ={res} /\ BIRO.IRO.mp{1} = RO.m{2}.
+proof.
+proc; inline*; sp.
+if{1}; sp.
++ rcondt{1} 1; auto=> /=/>.
+  conseq(:_==> take k{1} bs{1} = l{2} /\ BIRO.IRO.mp{1} = RO.m{2}).
+  * smt().
+  case: (0 <= n{2}); last first.
+  + rcondf{2} 1; 1: by auto; smt(). 
+    conseq(:_==> BIRO.IRO.mp{1} = RO.m{2} /\ ={i} /\ n{1} = size_out /\ x2{1} = x0{2})=> />.
+    - smt(take_le0).
+    while(={i} /\ x2{1} = x0{2} /\ n{1} = size_out /\ BIRO.IRO.mp{1} = RO.m{2}).
+    - sp; if{1}.
+      - by rcondt{2} 2; auto=> />.
+      by rcondf{2} 2; auto=> />; smt(dbool_ll).
+    by auto=> />.
+  splitwhile{1} 1 : i < k.
+  while(={i} /\ n{1} = size_out /\ x2{1} = x0{2} /\  BIRO.IRO.mp{1} = RO.m{2} /\
+      take k{1} bs{1} = l{2} /\ size bs{1} = i{1} /\ k{1} <= i{1} <= size_out).
+  * sp; if{1}.
+    - by rcondt{2} 2; auto; smt(dbool_ll cats1 take_cat cats0 take_size size_rcons).
+    by rcondf{2} 2; auto; smt(dbool_ll cats1 take_cat cats0 take_size size_rcons).
+  conseq(:_==> ={i} /\ n{1} = size_out /\ x2{1} = x0{2} /\  BIRO.IRO.mp{1} = RO.m{2} /\
+      bs{1} = l{2} /\ size bs{1} = i{1} /\ k{1} = i{1}).
+  + smt(take_size).
+  while(={i} /\ x2{1} = x0{2} /\ n{1} = size_out /\ k{1} = n{2} /\
+      0 <= i{1} <= k{1} <= size_out /\ bs{1} = l{2} /\ size bs{1} = i{1} /\
+      BIRO.IRO.mp{1} = RO.m{2}).
+  + sp; if{1}.
+    - by rcondt{2} 2; auto; smt(size_rcons).
+    by rcondf{2} 2; auto; smt(size_rcons dbool_ll).
+  by auto; smt(size_ge0 size_out_gt0).
+rcondt{1} 1; auto.
+rcondf{2} 2; 1: auto.
++ conseq(:_==> i = n); 1: smt().
+  by while(i <= n); auto=> />; smt(size_out_gt0).
+while(i0{1} = i{2} /\ x3{1} = x0{2} /\ n0{1} = n{2} /\ bs0{1} = l{2} /\ 
+    BIRO.IRO.mp{1} = RO.m{2}).
++ sp; if{1}.
+  - by rcondt{2} 2; auto=> />.
+  by rcondf{2} 2; auto; smt(dbool_ll).
+by auto=> />.
+qed.
+
+local module Dist (F : RO) = {
+  proc distinguish = SHA3_OIndiff.OIndif.OIndif(FSome(Fill_In(F)),
+      OSimulator(FSome(Fill_In(F))), ODRestr(Dist_of_P1Adv(A))).main
+}.
+
+local module Game (F : RO) = {
+  proc distinguish () = {
+    var bo;
+    OSimulator(FSome(Fill_In(F))).init();
+    Counter.c <- 0;
+    Log.m <- empty;
+    F.init();
+    bo <@ Dist(F).distinguish();
+    return bo;
+  }
+}.
+
+local lemma eager_ideal &m :
+    Pr[SHA3_OIndiff.OIndif.OIndif(FSome(BIRO.IRO),
+      OSimulator(FSome(BIRO.IRO)),
+      ODRestr(Dist_of_P1Adv(A))).main() @ &m : res] =
+    Pr[SHA3_OIndiff.OIndif.OIndif(ExtendSample(FSome(BIRO.IRO)),
+      OSimulator(ExtendSample(FSome(BIRO.IRO))),
+      ODRestr(Dist_of_P1Adv(A))).main() @ &m : res].
+proof.
+cut->: 
+  Pr[SHA3_OIndiff.OIndif.OIndif(FSome(BIRO.IRO),
+    OSimulator(FSome(BIRO.IRO)),
+    ODRestr(Dist_of_P1Adv(A))).main() @ &m : res] =
+  Pr[Game(LRO).distinguish() @ &m : res].
++ byequiv=> //=; proc.
+  inline{2} 1; sp; inline{2} 1; sp; inline{2} 1; sp; inline{2} 1; sp.
+  inline{1} 1; inline{2} 1; sp.
+  inline{1} 1; inline{2} 1; sp.
+  inline{1} 1; inline{2} 1; sp.
+  inline{1} 1; inline{2} 1; sp.
+  inline{1} 1; inline{2} 1; sp.
+  inline{1} 1; inline{2} 1; sp; sim.
+  seq 2 2 : (={hash, m, glob OFC} /\ BIRO.IRO.mp{1} = RO.m{2}); last first.
+  - inline{1} 1; inline{2} 1; sp; sim.
+    inline{1} 1; inline{2} 1; sp; sim; if; auto.
+    inline{1} 1; inline{2} 1; sp; sim.
+    by call eq_eager_ideal; auto.
+  call(: ={glob OFC, glob OSimulator} /\ BIRO.IRO.mp{1} = RO.m{2}); auto.
+  - proc; sp; if; auto.
+    inline{1} 1; inline{2} 1; sp; sim; if; 1: auto; sim.
+    if; 1: auto; sim; sp.
+    if; 1: auto; 1: smt(); sim.
+    * inline{1} 1; inline{2} 1; sp; sim.
+      by call eq_eager_ideal; auto; smt().
+    smt().
+  - by proc; inline*; sim.
+  proc; sim.
+  inline{1} 1; inline{2} 1; sp; sim; if; 1: auto; sim.
+  inline{1} 1; inline{2} 1; sp; sim.
+  by call eq_eager_ideal; auto.
+cut->: 
+  Pr[SHA3_OIndiff.OIndif.OIndif(ExtendSample(FSome(BIRO.IRO)),
+    OSimulator(ExtendSample(FSome(BIRO.IRO))),
+    ODRestr(Dist_of_P1Adv(A))).main() @ &m : res] =
+  Pr[Game(RO).distinguish() @ &m : res].
++ byequiv=>//=; proc.
+  inline{2} 1; sp; inline{2} 1; sp; inline{2} 1; sp; inline{2} 1; sp.
+  inline{1} 1; inline{2} 1; sp.
+  inline{1} 1; inline{2} 1; sp.
+  inline{1} 1; inline{2} 1; sp.
+  inline{1} 1; inline{2} 1; sp.
+  inline{1} 1; inline{2} 1; sp.
+  inline{1} 1; inline{2} 1; sp; sim.
+  seq 2 2 : (={hash, m, glob OFC} /\ BIRO.IRO.mp{1} = RO.m{2}); last first.
+  - inline{1} 1; inline{2} 1; sp; sim.
+    inline{1} 1; inline{2} 1; sp; sim; if; auto.
+    by call eq_eager_ideal2; auto.
+  call(: ={glob OFC, glob OSimulator} /\ BIRO.IRO.mp{1} = RO.m{2}); auto.
+  - proc; sp; if; auto.
+    inline{1} 1; inline{2} 1; sp; sim; if; 1: auto; sim.
+    if; 1: auto; sim; sp.
+    if; 1: auto; 1: smt(); sim.
+    * by call eq_eager_ideal2; auto; smt().
+    smt().
+  - by proc; inline*; sim.
+  proc; sim.
+  inline{1} 1; inline{2} 1; sp; sim; if; 1: auto; sim.
+  by call eq_eager_ideal2; auto.
+rewrite eq_sym; byequiv=> //=; proc. 
+call(RO_LRO_D Dist); inline*; auto=> />.
+qed.
+
+
 
 
 local lemma rw_ideal_2 &m:
@@ -454,20 +680,26 @@ have->:Pr[SORO.Preimage(SORO_P1(A), RFList).main() @ &m : res] =
   inline{1} 1; inline{2} 1; sp; sim.
   inline{1} 1; inline{2} 1; sp; if; auto; sim.
   by call(rw_RF_List_While); auto.
-have->:Pr[SHA3_OIndiff.OIndif.OIndif(FSome(BIRO.IRO),
-         OSimulator(FSome(BIRO.IRO)),
+rewrite (eager_ideal &m).
+have->:Pr[SHA3_OIndiff.OIndif.OIndif(ExtendSample(FSome(BIRO.IRO)),
+         OSimulator(ExtendSample(FSome(BIRO.IRO))),
           ODRestr(Dist_of_P1Adv(A))).main() @ &m : res] =
-       Pr[SHA3_OIndiff.OIndif.OIndif(FSome(BIRO.IRO),
+       Pr[SHA3_OIndiff.OIndif.OIndif(ExtendSample(FSome(BIRO.IRO)),
          OSimulator(ExtendOutputSize(FSetSize(FSome(BIRO.IRO)))),
          ODRestr(Dist_of_P1Adv(A))).main() @ &m : res].
 + byequiv=> //=; proc; inline*; sp.
   seq 2 2 : (={m, hash, glob OSimulator, glob OFC} /\
          eq_extend_size BIRO.IRO.mp{1} BIRO.IRO.mp{2} Log.m{2}); last first.
-  - sp; if; auto; sp; if; auto.
-    while(={i, n, x1, bs} /\ eq_extend_size BIRO.IRO.mp{1} BIRO.IRO.mp{2} Log.m{2} /\
-         n{1} = size_out /\ 0 <= i{1} <= n{1}); auto.
-    * by sp; if; auto; smt(domE get_setE). 
-    by move=> /> &l &r Heq1 Heq2 Heq3 Hc Hvalid; smt(size_out_gt0).
+  - sp; if; auto; sp; if; auto; sp; rcondt{1}1; 1: auto. 
+    * rcondt{2} 1; 1: auto.
+      while(={i, n, bs, x3} /\ size bs{1} = i{1} /\
+           eq_extend_size BIRO.IRO.mp{1} BIRO.IRO.mp{2} Log.m{2} /\
+           n{1} = size_out /\ 0 <= i{1} <= n{1}); auto.
+      * by sp; if; auto; smt(domE get_setE size_rcons).
+      smt(size_out_gt0 take_oversize size_out_gt0).
+    * by auto; rcondf{1} 1; auto.
+    * rcondt{2} 1; 1: auto; move=> />; auto.
+      by while(={i0, n0}); auto; sp; if{1}; if{2}; auto; smt(dbool_ll).
   call(: ={glob OSimulator, glob OFC} /\
          eq_extend_size BIRO.IRO.mp{1} BIRO.IRO.mp{2} Log.m{2}); last first; auto.
   + smt(mem_empty).
@@ -478,8 +710,18 @@ have->:Pr[SHA3_OIndiff.OIndif.OIndif(FSome(BIRO.IRO),
     - by conseq=> />; sim; smt().
     wp=> />; 1: smt().
     rnd; auto=> />; 1: smt().
-    call(: eq_extend_size BIRO.IRO.mp{1} BIRO.IRO.mp{2} Log.m{2}); last by auto; smt().
-
+    call(eq_extend); last by auto; smt().
+  + by proc; sp; if; auto; inline{1} 1; inline{2} 1; sp; if; auto.
+  proc; sp; inline{1} 1; inline{2} 1; sp; if; auto.
+  inline*; sp.
+  rcondt{1} 1; 1: auto; rcondt{2} 1; 1: auto; sp.
+  rcondt{1} 1; 1: auto; rcondt{2} 1; 1: auto; sp; auto.
+  conseq(:_==> ={bs} /\ eq_extend_size BIRO.IRO.mp{1} BIRO.IRO.mp{2} Log.m{2}); 
+    1: by auto.
+  while(={i, n, x3, bs} /\ 0 <= i{1} <= size_out /\ n{1} = size_out /\ 
+      eq_extend_size BIRO.IRO.mp{1} BIRO.IRO.mp{2} Log.m{2}).
+  - by sp; if; auto; smt(domE get_setE size_rcons).
+  by auto; smt(size_out_gt0).
 byequiv=> //=; proc.
 inline{1} 1; inline{2} 2; sp.
 inline{1} 1; inline{2} 3; swap{2}[1..2]1; sp.
@@ -487,8 +729,8 @@ inline{1} 1; inline{2} 3; sp.
 inline{1} 1; sp.
 inline{1} 1; sp.
 swap{2} 1 1; sp; swap{2}[1..2]3; sp.
-inline{1} 1; sp; auto. print ExtendOutputSize.
-seq 2 5 : (={glob A, glob OSimulator, glob Counter, hash, m} /\
+inline{1} 1; sp; auto. 
+seq 2 5 : (={glob A, glob OSimulator, glob Counter, glob Log, hash, m} /\
          inv BIRO.IRO.mp{1} RFList.m{2} /\
          SORO.Bounder.bounder{2} <= Counter.c{1}); last first.
 + inline{1} 1; inline{2} 1; sp; inline{1} 1; sp; auto.
@@ -498,22 +740,52 @@ seq 2 5 : (={glob A, glob OSimulator, glob Counter, hash, m} /\
     by while{2}(true)(size_out - i{2}); auto=>/>; smt(dbool_ll).
   rcondt{2} 1; 1: by auto=> />; smt(divz_ge0 gt0_r size_ge0).
   inline{1} 1; sp; auto.
-  auto; call(eq_IRO_RFWhile); auto.
-auto; call(: ={glob OSimulator, glob Counter} /\ inv BIRO.IRO.mp{1} RFList.m{2} /\
-        SORO.Bounder.bounder{2} <= Counter.c{1}); auto=> />.
-+ smt().
-+ proc; sp; if; auto=> />; 2: smt(); inline{1} 1; inline{2} 1; sp; auto.
+  rcondt{1} 1; auto=> /=. 
+  inline{1} 1; sp; auto.
+  by call(eq_IRO_RFWhile); auto; smt(take_oversize).
+auto; call(: ={glob OSimulator, glob Counter, glob Log} /\ 
+    inv BIRO.IRO.mp{1} RFList.m{2} /\
+    SORO.Bounder.bounder{2} <= Counter.c{1}); auto; last first.
++ by inline*; auto; smt(mem_empty).
++ proc; sp; if; auto=> />; 1: smt(). 
+  inline{1} 1; inline{2} 1; sp; auto.
   if; 1, 3: auto; -1: smt().
-  
-  (* TODO : reprendre ici, avec le spit des domaines *)
-
-
+  if; 1, 3: auto; -1: smt().
+  sp; if; 1: auto; 1: smt(); last first.
+  - by conseq(:_==> ={y, glob OSimulator}); 1: smt(); sim; smt().
+  inline{1} 1; inline{2} 1; sp.
+  inline{1} 1; inline{2} 1; sp.
+  rcondt{2} 1; 1: by auto; smt().
+  sp.
+  seq 3 2 : (={x0, x1, o1, k0, Log.m, suffix, glob OSimulator} /\
+      inv BIRO.IRO.mp{1} RFList.m{2} /\ 
+      SORO.Bounder.bounder{2} <= Counter.c{2} + 1); last first.
+  - by conseq(:_==> ={y, x1, glob OSimulator, Log.m}); 1: smt(); sim=> />.
+  inline{1} 1; auto.
+  by call(eq_IRO_RFWhile); auto; smt().
++ by proc; inline*; sp; if; auto; sp; if; auto=> />; smt().
+proc.
+inline{1} 1; inline{2} 1; sp; if; auto=> /=.
+inline{1} 1; inline{2} 1; sp.
+rcondt{1} 1; 1: auto.
+inline{1} 1; auto.
+rcondf{2} 4; 1: auto. 
++ inline*; auto; sp; if; auto; sp; if; auto=> />; conseq(:_==> true); 1: smt().
+  by while(true); auto.
+inline{2} 1; sp.
+rcondt{2} 1; 1: by auto; smt(divz_ge0 gt0_r size_ge0).
+auto; call eq_IRO_RFWhile; auto=> />.
+move=> &l &r 13?; split; 2: smt(divz_ge0 gt0_r size_ge0).
+rewrite 2!oget_some cats0 take_oversize 1:/# take_oversize 1:spec_dout //=.
+have h:=spec2_dout result_L H5.
+have-> := some_oget _ h.
+by rewrite eq_sym -to_listK; congr.
 qed.
 
 local lemma rw_ideal &m:
     Pr[SHA3_OIndiff.OIndif.OIndif(FSome(BIRO.IRO), OSimulator(FSome(BIRO.IRO)), 
       ODRestr(Dist_of_P1Adv(A))).main() @ &m : res] <=
-    Pr[SORO.Preimage(SORO_P1(A),RF(RO.RO)).main() @ &m : res].
+    Pr[SORO.Preimage(SORO_P1(A),RF(SORO.RO.RO)).main() @ &m : res].
 proof.
 rewrite (StdOrder.RealOrder.ler_trans _ _ _ (rw_ideal_2 &m)).
 byequiv(: ={glob A} ==> _) => //=; proc; inline*; sp; wp.
@@ -529,14 +801,41 @@ seq 2 2 : (
   RFList.m{1} = empty /\
   Counter.c{2} = 0 /\
   ={Log.m, glob SHA3Indiff.Simulator, glob SORO.Bounder, glob Counter} /\
-  RO.RO.m{2} = empty /\ ={glob A, h, hash}); 1: auto=> />. 
+  SORO.RO.RO.m{2} = empty /\ ={glob A, h, hash}); 1: auto=> />. 
 seq 1 1 : (={glob A, glob SHA3Indiff.Simulator, glob SORO.Bounder, glob Counter, 
-    mi, h, hash} /\ RFList.m{1} = RO.RO.m{2}).
-+ call(: ={glob SHA3Indiff.Simulator, glob SORO.Bounder, glob Counter} /\ 
-    RFList.m{1} = RO.RO.m{2}); auto.
-  - admit.
-  - admit.    
-  - admit.
+    glob Log, mi, h, hash} /\ RFList.m{1} = SORO.RO.RO.m{2}).
++ call(: ={glob SHA3Indiff.Simulator, glob SORO.Bounder, glob Counter, glob Log} /\ 
+    RFList.m{1} = SORO.RO.RO.m{2}); auto.
+  - proc; sp; if; 1, 3: auto; sp.
+    inline *; sp; sim.
+    if; 1: auto; sim. 
+    if; 1: auto; sim.
+    sp; if; 1: (auto; smt()); sim; 2: smt(). 
+    sp; if; 1: auto; sim; -1: smt().
+    sp; if{1}.
+    * rcondt{2} 2; auto; 1: smt(BlockSponge.parse_valid).
+      rnd (fun l => oget (of_list l)) to_list; auto=> />.
+      move=> &l &r 10?; split; 1: smt(of_listK).
+      rewrite -dout_equal_dlist=> ?; split=> ?.
+      + by rewrite dmapE=> h{h}; apply mu_eq=> x; smt(to_list_inj).
+      move=> sample.
+      rewrite !get_setE/=oget_some/=dout_full/= => h; split; 2: smt(). 
+      rewrite eq_sym to_listK; apply some_oget.
+      apply spec2_dout.
+      by move:h; rewrite supp_dmap; smt(spec_dout).
+    by auto; smt(dout_ll).
+  - by proc; inline*; sp; if; auto; sp; if; auto.
+  - proc; inline*; sp; if; auto; sp; if; auto; sp; sim.
+    if{1}.
+    * rcondt{2} 2; auto.
+      rnd (fun l => oget (of_list l)) to_list; auto=> />.
+      move=> &l 4?; split=> ?; 1: smt(of_listK).
+      rewrite -dout_equal_dlist; split=> ?.
+      * by rewrite dmapE=> h{h}; apply mu_eq=> x; smt(to_list_inj).
+      move=> sample.
+      rewrite supp_dmap dout_full/= =>/> a.
+      by rewrite get_setE/=oget_some/= dout_full/=; congr; rewrite of_listK oget_some.
+  by auto; smt(dout_ll).
 sp; if; 1, 3: auto; sp; wp 1 2.
 if{1}.
 + wp=> />.
@@ -564,12 +863,14 @@ local lemma leq_ideal &m :
     Pr[SHA3_OIndiff.OIndif.OIndif(FSome(BIRO.IRO), OSimulator(FSome(BIRO.IRO)), 
       ODRestr(Dist_of_P1Adv(A))).main() @ &m : res] <= (sigma + 1)%r / 2%r ^ size_out.
 proof.
-print SORO.RO_is_preimage_resistant. 
-have:=rw_ideal &m.
-admit.
+rewrite (StdOrder.RealOrder.ler_trans _ _ _ (rw_ideal &m)).
+rewrite (StdOrder.RealOrder.ler_trans _ _ _ (RO_is_preimage_resistant (SORO_P1(A)) &m)).
+by rewrite doutE1.
 qed.
 
-  local lemma rw_real &m (A <: SH.AdvPreimage { Perm, Counter, Bounder }): 
+
+
+  local lemma rw_real &m : 
       Pr[Preimage(A, OSponge, PSome(Perm)).main() @ &m : res] =
       Pr[SHA3_OIndiff.OIndif.OIndif(FSome(Sponge(Poget(PSome(Perm)))), PSome(Perm), 
         ODRestr(Dist_of_P1Adv(A))).main() @ &m : res].
@@ -595,7 +896,7 @@ lemma Sponge_preimage_resistant &m:
     (sigma + 1)%r / (2%r ^ size_out).
 proof.
 move=> A_ll.
-rewrite (rw_real &m A).
+rewrite (rw_real &m).
 have := SHA3OIndiff (Dist_of_P1Adv(A)) &m _.
 + move=> F P Hp Hpi Hf; proc; inline*; sp; auto; call Hf; auto. 
   call(A_ll (DFSetSize(F)) P _ Hp Hpi); auto.
@@ -604,1166 +905,788 @@ have := SHA3OIndiff (Dist_of_P1Adv(A)) &m _.
 by have/#:=leq_ideal &m.
 qed.
 
-
-(* old proof *)
-
-  declare module A : SH.AdvPreimage{SRO.RO.RO, SRO.RO.FRO, SRO.Bounder, Perm, 
-    Gconcl_list.BIRO2.IRO, Simulator, Cntr, BIRO.IRO, F.RO, F.FRO, Redo, C, 
-    Gconcl.S, BlockSponge.BIRO.IRO, BlockSponge.C, Gconcl_list.F2.RO,
-    Gconcl_list.F2.FRO, Gconcl_list.Simulator, DPre}.
-
-  axiom A_ll (F <: SRO.Oracle) : islossless F.get => islossless A(F).guess.
-
-  local lemma invm_dom_rng (m mi : (state, state) fmap) :
-      invm m mi => dom m = rng mi.
-  proof. 
-  move=>h; rewrite fun_ext=> x; rewrite domE rngE /= eq_iff; have h2 := h x; split.
-  + move=> m_x_not_None; exists (oget m.[x]); rewrite -h2; move: m_x_not_None.
-    by case: (m.[x]).
-  by move=> [] a; rewrite -h2 => ->.
-  qed.
-
-  local lemma invmC' (m mi : (state, state) fmap) :
-      invm m mi => invm mi m.
-  proof. by rewrite /#. qed.
-
-  local lemma invmC (m mi : (state, state) fmap) :
-      invm m mi <=> invm mi m.
-  proof. by split;exact invmC'. qed.
-
-  local lemma useful m mi a :
-      invm m mi => ! a \in m => Distr.is_lossless ((bdistr `*` cdistr) \ rng m).
-  proof.
-  move=>hinvm nin_dom.
-  cut prod_ll:Distr.is_lossless (bdistr `*` cdistr).
-  + by rewrite dprod_ll DBlock.dunifin_ll DCapacity.dunifin_ll. 
-  apply dexcepted_ll=>//=;rewrite-prod_ll.
-  cut->:predT = predU (predC (rng m)) (rng m);1:rewrite predCU//=.
-  rewrite Distr.mu_disjoint 1:predCI//=StdRing.RField.addrC. 
-  cut/=->:=StdOrder.RealOrder.ltr_add2l (mu (bdistr `*` cdistr) (rng m)) 0%r.
-  rewrite Distr.witness_support/predC.
-  move:nin_dom;apply absurd=>//=;rewrite negb_exists/==>hyp. 
-  cut{hyp}hyp:forall x, rng m x by smt(supp_dprod DBlock.supp_dunifin DCapacity.supp_dunifin). 
-  move:a. 
-  cut:=eqEcard (fdom m) (frng m);rewrite leq_card_rng_dom/=. 
-  cut->//=:fdom m \subset frng m. 
-  + by move=> x; rewrite mem_fdom mem_frng hyp.
-  smt(mem_fdom mem_frng).
-  qed.
-
-
-  local equiv equiv_sponge_perm c m :
-      FInit(CSetSize(Sponge, Perm)).get ~ FInit(DFSetSize(FC(Sponge(Perm)))).get :
-    ={arg, glob Perm} /\ invm Perm.m{1} Perm.mi{1} /\ 
-      Cntr.c{2} = c /\ arg{2} = m /\
-      (Cntr.c + ((size arg + 1) %/ Common.r + 1) + 
-      max ((size_out + Common.r - 1) %/ Common.r - 1) 0 <= limit){2} ==>
-    ={res, glob Perm} /\ invm Perm.m{1} Perm.mi{1} /\ 
-      Cntr.c{2} = c + ((size m + 1) %/ Common.r + 1) + 
-      max ((size_out + Common.r - 1) %/ Common.r - 1) 0.
-  proof.
-  proc; inline FC(Sponge(Perm)).f; sp.
-  rcondt{2} 1; auto; sp.
-  call(: ={glob Perm} /\ invm Perm.m{1} Perm.mi{1})=>/=; auto; inline*.
-  while(={i, n, sa, sc, z, glob Perm} /\ invm Perm.m{1} Perm.mi{1}); auto.
-  + sp; if; auto; sp; if; auto; progress.
-    rewrite invm_set //=.
-    by move:H4; rewrite supp_dexcepted.
-  sp; conseq(:_==> ={i, n, sa, sc, glob Perm} /\ invm Perm.m{1} Perm.mi{1}); auto.
-  while(={xs, sa, sc, glob Perm} /\ invm Perm.m{1} Perm.mi{1}); auto.
-  sp; if; auto; progress. 
-  rewrite invm_set=>//=.
-  by move:H4; rewrite supp_dexcepted.
-  qed.
-
-
-  op same_ro (m1 : (bool list, f_out) fmap) (m2 : (bool list * int, bool) fmap) =
-      (forall m, m \in m1 => forall i, 0 <= i < size_out => (m,i) \in m2)
-    && (forall m, (exists i, 0 <= i < size_out /\ (m,i) \in m2) => m \in m1)
-    && (forall m, m \in m1 => to_list (oget m1.[m]) = map (fun i => oget m2.[(m,i)]) (range 0 size_out)).
-
-  op same_ro2 (m1 : (bool list, bool list) fmap) (m2 : (bool list * int, bool) fmap) =
-      (forall m, m \in m1 => forall i, 0 <= i < size_out => (m,i) \in m2)
-    && (forall m, (exists i, 0 <= i < size_out /\ (m,i) \in m2) => m \in m1)
-    && (forall m, m \in m1 => oget m1.[m] = map (fun i => oget m2.[(m,i)]) (range 0 size_out)).
-
-  clone import Program as Prog with
-    type t <- bool,
-    op d <- dbool
-    proof *.
-
-  local equiv equiv_ro_iro c m :
-    FInit(RO).get ~ FInit(DFSetSize(FC(BIRO.IRO))).get :
-    ={arg} /\ same_ro SRO.RO.RO.m{1} BIRO.IRO.mp{2} /\
-    arg{2} = m /\ Cntr.c{2} = c /\
-    (Cntr.c + ((size arg + 1) %/ Common.r + 1) + 
-      max ((size_out + Common.r - 1) %/ Common.r - 1) 0 <= limit){2}
-    ==> ={res} /\ same_ro SRO.RO.RO.m{1} BIRO.IRO.mp{2} /\ 
-      Cntr.c{2} = c + ((size m + 1) %/ Common.r + 1) + 
-      max ((size_out + Common.r - 1) %/ Common.r - 1) 0.
-  proof.
-  proc; inline *; sp; rcondt{2} 1; 1: auto.
-  swap{2} 1 5; sp; wp 2 1.
-  conseq(:_==> oget SRO.RO.RO.m{1}.[x{1}] = oget (of_list bs0{2}) /\
-    same_ro SRO.RO.RO.m{1} BIRO.IRO.mp{2}); 1:by auto.
-  rcondt{2} 1; 1: auto.
-  case: (x{1} \in SRO.RO.RO.m{1}).
-  + rcondf{1} 2; auto.
-    exists* BIRO.IRO.mp{2}; elim* => mp.
-    while{2}(bs0{2} = map (fun j => oget BIRO.IRO.mp{2}.[(x0{2},j)]) (range 0 i{2})
-        /\ n0{2} = size_out /\ x0{2} \in SRO.RO.RO.m{1} /\ 0 <= i{2} <= size_out
-        /\ same_ro SRO.RO.RO.m{1} BIRO.IRO.mp{2} /\ BIRO.IRO.mp{2} = mp)
-      (size_out - i{2}); auto.
-    - sp; rcondf 1; auto; 1: smt().
-      progress. 
-      * have/=<-:= map_rcons (fun (j : int) => oget BIRO.IRO.mp{hr}.[(x0{hr}, j)]) (range 0 i{hr}) i{hr}.
-        by rewrite !rangeSr //=.
-      * smt().
-      * smt().
-      * smt().
-    progress. 
-    - by rewrite range_geq.
-    - smt(size_out_gt0).
-    - smt().
-    - exact(dout_ll).
-    - have[] h[#] h1 h2 := H.
-      cut->:i_R = size_out by smt().
-      cut<-:=h2 _ H3.
-      smt(to_listK).
-  rcondt{1} 2; 1: auto; wp =>/=.
-  exists* BIRO.IRO.mp{2}; elim* => mp.
-  conseq(:_==> 
-        same_ro SRO.RO.RO.m{1} mp /\ i{2} = size_out /\
-        (forall (l,j),  (l,j) \in mp => (l,j) \in BIRO.IRO.mp{2}) /\
-        (forall (l,j),  (l,j) \in mp => BIRO.IRO.mp{2}.[(l,j)] = mp.[(l,j)]) /\
-        (forall (l,j), (l,j) \in BIRO.IRO.mp{2} => (l,j) \in mp \/ (l = x0{2} /\ 0 <= j < i{2})) /\
-        (forall j, 0 <= j < i{2} => (x0{2},j) \in BIRO.IRO.mp{2}) /\
-        take i{2} (to_list r{1}) = bs0{2} /\
-        take i{2} (to_list r{1}) = map (fun (j : int) => oget BIRO.IRO.mp{2}.[(x0{2}, j)]) (range 0 i{2})); progress=>//=.
-  + by rewrite get_set_sameE /= oget_some; smt(to_listK take_oversize spec_dout).
-  + move:H8; rewrite mem_set=>[][]//=h; 1:rewrite H3=>//=.
-    - by have []h1 []h2 h3:= H2; have->//:=h1 _ h.
-    by move:h => <<-; rewrite H6 //=.
-  + rewrite mem_set//=; have[]//=h:= H5 _ _ H11; left.
-    have []h1 []->//=:= H2.
-    by exists i0=>//=.
-  + move:H7; rewrite take_oversize 1:spec_dout//= => H7.
-    move:H10; rewrite mem_set. 
-    case(m \in SRO.RO.RO.m{1})=>//=h.
-    - rewrite get_set_neqE; 1:smt().
-      have []h1 []h2 ->//=:= H2. 
-      by apply eq_in_map=> j;rewrite mem_range=>[][]hj1 hj2/=; rewrite H4//=h1//=.
-    by move=><<-; rewrite get_set_eqE//=.
-  alias{1} 1 l = [<:bool>].
-  transitivity{1} {
-      l <@ Sample.sample(size_out);
-      r <- oget (of_list l);
-    }
-    (={glob SRO.RO.RO, x} ==> ={glob SRO.RO.RO, r})
-    (x{1} = x0{2} /\ i{2} = 0 /\ n0{2} = size_out /\ mp = BIRO.IRO.mp{2} /\
-      same_ro SRO.RO.RO.m{1} BIRO.IRO.mp{2} /\ x{1} \notin SRO.RO.RO.m{1} /\
-      bs0{2} = []
-      ==>
-      same_ro SRO.RO.RO.m{1} mp /\ i{2} = size_out /\
-      (forall (l,j),  (l,j) \in mp => (l,j) \in BIRO.IRO.mp{2}) /\
-      (forall (l,j),  (l,j) \in mp => BIRO.IRO.mp{2}.[(l,j)] = mp.[(l,j)]) /\
-      (forall (l,j), (l,j) \in BIRO.IRO.mp{2} => (l,j) \in mp \/ (l = x0{2} /\ 0 <= j < i{2})) /\
-      (forall j, 0 <= j < i{2} => (x0{2},j) \in BIRO.IRO.mp{2}) /\
-      take i{2} (to_list r{1}) = bs0{2} /\
-      take i{2} (to_list r{1}) = 
-        map (fun (j : int) => oget BIRO.IRO.mp{2}.[(x0{2}, j)]) (range 0 i{2})); 
-    progress.
-  + smt().
-  + inline*; sp; wp. 
-    rnd to_list (fun x => oget (of_list x)); auto; progress. 
-    - smt(spec_dout supp_dlist to_listK spec2_dout size_out_gt0). 
-    - rewrite -dout_equal_dlist dmap1E; apply mu_eq=> x/=. 
-      smt(to_listK).
-    - rewrite-dout_equal_dlist supp_dmap; smt(dout_full).
-    smt(to_listK).
-  wp=>/=.
-  conseq(:_==> i{2} = size_out /\ size l{1} = size_out /\
-      (forall (l0 : bool list) (j : int),
-        (l0, j) \in mp => (l0, j) \in BIRO.IRO.mp{2}) /\
-      (forall (l0 : bool list) (j : int),
-        (l0, j) \in mp => BIRO.IRO.mp{2}.[(l0, j)] = mp.[(l0, j)]) /\
-      (forall (l0 : bool list) (j : int),
-        (l0, j) \in BIRO.IRO.mp{2} => ((l0, j) \in mp) \/ (l0 = x0{2} /\ 0 <= j < i{2})) /\
-      (forall (j : int), 0 <= j < i{2} => (x0{2}, j) \in BIRO.IRO.mp{2}) /\
-      take i{2} l{1} = bs0{2} /\
-      take i{2} l{1} =
-        map (fun (j : int) => oget BIRO.IRO.mp{2}.[(x0{2}, j)]) (range 0 i{2}));
-    progress.
-  + have[]//=h h1:=to_listK (oget (of_list l_L)) l_L; rewrite h1//==> {h1 h}.
-    smt(spec2_dout).
-  + have[]//=h h1:=to_listK (oget (of_list l_L)) l_L; rewrite h1//==> {h1 h}.
-    smt(spec2_dout). 
-  transitivity{1} {
-      l <@ LoopSnoc.sample(size_out);
-    }
-    (={glob SRO.RO.RO} ==> ={glob SRO.RO.RO, l})
-    (x{1} = x0{2} /\ i{2} = 0 /\ n0{2} = size_out /\ mp = BIRO.IRO.mp{2} /\
-      same_ro SRO.RO.RO.m{1} BIRO.IRO.mp{2} /\ x0{2} \notin SRO.RO.RO.m{1} /\
-      bs0{2} = []
-      ==>
-      i{2} = size_out /\ size l{1} = size_out /\
-      (forall (l,j),  (l,j) \in mp => (l,j) \in BIRO.IRO.mp{2}) /\
-      (forall (l,j),  (l,j) \in mp => BIRO.IRO.mp{2}.[(l,j)] = mp.[(l,j)]) /\
-      (forall (l,j), (l,j) \in BIRO.IRO.mp{2} => (l,j) \in mp \/ (l = x0{2} /\ 0 <= j < i{2})) /\
-      (forall j, 0 <= j < i{2} => (x0{2},j) \in BIRO.IRO.mp{2}) /\
-      take i{2} l{1} = bs0{2} /\
-      take i{2} l{1} = 
-        map (fun (j : int) => oget BIRO.IRO.mp{2}.[(x0{2}, j)]) (range 0 i{2})); 
-    progress.
-  + smt(). 
-  + by call Sample_LoopSnoc_eq; auto.
-  inline*; sp; wp.
-  conseq(:_==> i{2} = size_out /\ size l0{1} = i{2} /\ 
-      same_ro SRO.RO.RO.m{1} mp /\ x0{2} \notin SRO.RO.RO.m{1} /\
-      (forall l j, (l,j) \in mp => (l,j) \in BIRO.IRO.mp{2}) /\
-      (forall l j, (l,j) \in mp => BIRO.IRO.mp{2}.[(l, j)] = mp.[(l, j)]) /\
-      (forall l j, (l, j) \in BIRO.IRO.mp{2} => ((l, j) \in mp) \/ (l = x0{2} /\ 0 <= j < i{2})) /\
-      (forall j, 0 <= j < i{2} => (x0{2}, j) \in BIRO.IRO.mp{2}) /\
-      l0{1} = bs0{2} /\ bs0{2} = 
-        map (fun (j : int) => oget BIRO.IRO.mp{2}.[(x0{2}, j)]) (range 0 i{2})); progress.
-  + smt(take_oversize).
-  + smt(take_oversize).
-  while(0 <= i{2} <= size_out /\ size l0{1} = i{2} /\ n0{2} = size_out /\
-      ={i} /\ n{1} = n0{2} /\
-      same_ro SRO.RO.RO.m{1} mp /\ x0{2} \notin SRO.RO.RO.m{1} /\
-      (forall l j, (l,j) \in mp => (l,j) \in BIRO.IRO.mp{2}) /\
-      (forall l j, (l,j) \in mp => BIRO.IRO.mp{2}.[(l, j)] = mp.[(l, j)]) /\
-      (forall l j, (l, j) \in BIRO.IRO.mp{2} => ((l, j) \in mp) \/ (l = x0{2} /\ 0 <= j < i{2})) /\
-      (forall j, 0 <= j < i{2} => (x0{2}, j) \in BIRO.IRO.mp{2}) /\
-      l0{1} = bs0{2} /\ bs0{2} = 
-        map (fun (j : int) => oget BIRO.IRO.mp{2}.[(x0{2}, j)]) (range 0 i{2})).
-  + sp; wp=> //=.
-    rcondt{2} 1; 1:auto; progress.
-    - have[]h1 [] h2 h3 := H1.
-      have:=h2 x0{hr}; rewrite H2/= negb_exists/= =>/(_ (size bs0{hr})).
-      rewrite size_ge0 H9/=; apply absurd =>/= h.
-      by have //=:= H5 _ _ h.
-    rnd; auto; progress.
-    - smt(size_ge0).
-    - smt().
-    - by rewrite size_cat/=.
-    - by rewrite mem_set; left; rewrite H3. 
-    - rewrite get_setE (H4 _ _ H12).
-      cut/#: !(l1, j) = (x0{2}, size bs0{2}).
-      move:H2; apply absurd=> //=[#] <<- ->>.
-      have[] h1 [] h2 h3 := H1.
-      by apply h2; smt().
-    - move:H12; rewrite mem_set.
-      case((l1, j) \in BIRO.IRO.mp{2})=>//= h; 1: smt().
-      by move=> [#] <<- ->> //=; rewrite size_ge0; smt().
-    - rewrite mem_set.
-      case(j = size bs0{2})=>//=.
-      move=> h; rewrite h /=; have {H13} H13 {h} : j < size bs0{2} by smt().
-      by apply H6. 
-    - by rewrite cats1 get_set_sameE oget_some. 
-    - rewrite get_set_sameE oget_some H7 rangeSr.
-      rewrite !size_map 1:size_ge0. 
-      rewrite (size_map _ (range 0 (size bs0{2}))) size_range /=.
-      rewrite max_ler 1:size_ge0 map_rcons /=get_set_sameE oget_some; congr.
-      apply eq_in_map=> j.
-      rewrite mem_range /==> [] [] hj1 hj2.
-      by rewrite get_set_neqE //=; smt().
-  auto; progress.
-  + smt(size_out_gt0).
-  + smt().
-  + smt(). 
-  + by rewrite range_geq.
-  smt().
-  qed.
-
-  lemma Sponge_preimage_resistant &m ha :
-      (DPre.h{m} = ha) =>
-      Pr[SRO.Preimage(A, FM(CSetSize(Sponge), Perm)).main(ha) @ &m : res] <=
-      (limit ^ 2 - limit)%r / (2 ^ (r + c + 1))%r +
-      (4 * limit ^ 2)%r / (2 ^ c)%r +
-      (sigma + 1)%r / (2%r ^ size_out).
-  proof.
-  move=>init_ha.
-  rewrite -(doutE1 ha).
-  rewrite(preimage_resistant_if_indifferentiable A A_ll (CSetSize(Sponge)) Perm &m ha init_ha).
-  exists (SimSetSize(Simulator))=>//=; split.
-  + by move=> F _; proc; inline*; auto.
-  cut->//:Pr[Indiff0.Indif(CSetSize(Sponge, Perm), Perm, DPre(A)).main() @ &m : res] =
-        Pr[RealIndif(Sponge, Perm, DRestr(DSetSize(DPre(A)))).main() @ &m : res].
-  + byequiv=>//=; proc. 
-    inline DPre(A, CSetSize(Sponge, Perm), Perm).distinguish.
-    inline SRO.Preimage(A, FInit(CSetSize(Sponge, Perm))).main.
-    inline DRestr(DSetSize(DPre(A)), Sponge(Perm), Perm).distinguish 
-          DSetSize(DPre(A), FC(Sponge(Perm)), PC(Perm)).distinguish 
-          SRO.Preimage(A, FInit(DFSetSize(FC(Sponge(Perm))))).main.
-    inline Perm.init CSetSize(Sponge, Perm).init Sponge(Perm).init 
-          FC(Sponge(Perm)).init SRO.Counter.init Cntr.init 
-          SRO.Bounder(FInit(CSetSize(Sponge, Perm))).init 
-          SRO.Bounder(FInit(DFSetSize(FC(Sponge(Perm))))).init
-          FInit(CSetSize(Sponge, Perm)).init 
-          FInit(DFSetSize(FC(Sponge(Perm)))).init; sp. 
-    wp; sp; sim.
-    seq 1 1 : (={m, hash, glob DPre, glob SRO.Counter, glob Perm}
-          /\ invm Perm.m{1} Perm.mi{1} /\ DPre.h{1} = ha
-          /\ ={c}(SRO.Counter,Cntr)); last first.
-    - if; auto; sp.
-      exists* m{1}, SRO.Counter.c{1}; elim* => mess c.
-      by call(equiv_sponge_perm c mess); auto; smt().
-    call(: ={glob SRO.Counter, glob Perm, glob DPre, glob SRO.Bounder}
-          /\ DPre.h{1} = ha
-          /\ invm Perm.m{1} Perm.mi{1} /\ ={c}(SRO.Counter,Cntr)).
-    + proc; sp; if; auto; sp; if; auto; sp.
-      exists * x{1}; elim* => m c1 c2 b1 b2.
-      by call(equiv_sponge_perm c1 m); auto; smt().
-    auto; progress.
-    by rewrite /invm=> x y; rewrite 2!emptyE.
-  cut->//:Pr[Indiff0.Indif(RO, SimSetSize(Simulator, RO), DPre(A)).main() @ &m : res] =
-        Pr[IdealIndif(BIRO.IRO, Simulator, DRestr(DSetSize(DPre(A)))).main() @ &m : res].
-  + byequiv=>//=; proc.
-    inline Simulator(FGetSize(RO)).init RO.init Simulator(BIRO.IRO).init 
-          BIRO.IRO.init Gconcl_list.BIRO2.IRO.init; sp.
-    inline DPre(A, RO, Simulator(FGetSize(RO))).distinguish.
-    inline DRestr(DSetSize(DPre(A)), BIRO.IRO, Simulator(BIRO.IRO)).distinguish 
-          DSetSize(DPre(A), FC(BIRO.IRO), PC(Simulator(BIRO.IRO))).distinguish; wp; sim.
-    inline SRO.Bounder(FInit(DFSetSize(FC(BIRO.IRO)))).init 
-          SRO.Bounder(FInit(RO)).init SRO.Counter.init FInit(RO).init
-          FInit(DFSetSize(FC(BIRO.IRO))).init Cntr.init; sp.
-    inline SRO.Preimage(A, FInit(RO)).main 
-          SRO.Preimage(A, FInit(DFSetSize(FC(BIRO.IRO)))).main.
-    inline SRO.Counter.init SRO.Bounder(FInit(RO)).init 
-          SRO.Bounder(FInit(DFSetSize(FC(BIRO.IRO)))).init
-          FInit(RO).init FInit(DFSetSize(FC(BIRO.IRO))).init ; sp; sim.
-    seq 1 1 : (={m, glob SRO.Counter, glob DPre, hash}
-          /\ ={c}(SRO.Counter,Cntr) /\ DPre.h{1} = hash{1}
-          /\ same_ro SRO.RO.RO.m{1} BIRO.IRO.mp{2}); last first.
-    - if; auto; sp.
-      exists * m{1}, SRO.Counter.c{1}; elim* => mess c.
-      by call(equiv_ro_iro c mess); auto; smt().
-    conseq(:_==> ={m, glob SRO.Counter, glob SRO.Bounder, glob DPre}
-          /\ ={c}(SRO.Counter,Cntr)
-          /\ same_ro SRO.RO.RO.m{1} BIRO.IRO.mp{2}); progress.
-    call(: ={glob SRO.Counter, glob SRO.Bounder, glob DPre}
-          /\ ={c}(SRO.Counter,Cntr)
-          /\ same_ro SRO.RO.RO.m{1} BIRO.IRO.mp{2}); auto.
-    + proc; sp; if; auto; sp; if; auto; sp.
-      exists* x{1}; elim* => a c1 c2 b1 b2.
-      call(equiv_ro_iro c1 a); auto; smt().
-    smt(mem_empty).
-  have->//=:= SHA3Indiff (DSetSize(DPre(A))) &m _.
-  move=> F P P_f_ll P_fi_ll F_ll; proc; inline*; auto; sp; auto.
-  seq 1 : true; auto. 
-  + call (A_ll (SRO.Bounder(FInit(DFSetSize(F))))); auto.
-    by proc; inline*; sp; if; auto; sp; if; auto; sp; call F_ll; auto.
-  if; auto; sp.
-  by call F_ll; auto.
-  qed.
-
 end section Preimage.
 
 
 
 section SecondPreimage.
 
-  declare module A : SRO.AdvSecondPreimage{SRO.RO.RO, SRO.RO.FRO, SRO.Bounder, Perm, 
-    Gconcl_list.BIRO2.IRO, Simulator, Cntr, BIRO.IRO, F.RO, F.FRO, Redo, C, 
-    Gconcl.S, BlockSponge.BIRO.IRO, BlockSponge.C, Gconcl_list.F2.RO,
-    Gconcl_list.F2.FRO, Gconcl_list.Simulator, D2Pre}.
 
-  axiom A_ll (F <: SRO.Oracle) : islossless F.get => islossless A(F).guess.
+  declare module A : SH.AdvSecondPreimage { Perm, Counter, Bounder, F.RO,
+    F.FRO, Redo, C, Gconcl.S, BlockSponge.BIRO.IRO, BlockSponge.C, BIRO.IRO,
+    Gconcl_list.BIRO2.IRO, Gconcl_list.F2.RO, Gconcl_list.F2.FRO,
+    Gconcl_list.Simulator, SHA3Indiff.Simulator, SHA3Indiff.Cntr,
+    SORO.Bounder, SORO.RO.RO, RO, FRO }.
 
-  local lemma invm_dom_rng (m mi : (state, state) fmap) :
-      invm m mi => dom m = rng mi.
-  proof. 
-  move=>h; rewrite fun_ext=> x; rewrite domE rngE /= eq_iff; have h2 := h x; split.
-  + move=> m_x_not_None; exists (oget m.[x]); rewrite -h2; move: m_x_not_None.
-    by case: (m.[x]).
-  by move=> [] a; rewrite -h2 => ->.
-  qed.
+  local module FInit (F : OIndif.ODFUNCTIONALITY) : OIndif.OFUNCTIONALITY = {
+    proc init () = {}
+    proc f = F.f
+  }.
 
-  local lemma invmC' (m mi : (state, state) fmap) :
-      invm m mi => invm mi m.
-  proof. by rewrite /#. qed.
-
-  local lemma invmC (m mi : (state, state) fmap) :
-      invm m mi <=> invm mi m.
-  proof. by split;exact invmC'. qed.
-
-  local lemma useful m mi a :
-      invm m mi => ! a \in m => Distr.is_lossless ((bdistr `*` cdistr) \ rng m).
-  proof.
-  move=>hinvm nin_dom.
-  cut prod_ll:Distr.is_lossless (bdistr `*` cdistr).
-  + by rewrite dprod_ll DBlock.dunifin_ll DCapacity.dunifin_ll. 
-  apply dexcepted_ll=>//=;rewrite-prod_ll.
-  cut->:predT = predU (predC (rng m)) (rng m);1:rewrite predCU//=.
-  rewrite Distr.mu_disjoint 1:predCI//=StdRing.RField.addrC. 
-  cut/=->:=StdOrder.RealOrder.ltr_add2l (mu (bdistr `*` cdistr) (rng m)) 0%r.
-  rewrite Distr.witness_support/predC.
-  move:nin_dom;apply absurd=>//=;rewrite negb_exists/==>hyp. 
-  cut{hyp}hyp:forall x, rng m x by smt(supp_dprod DBlock.supp_dunifin DCapacity.supp_dunifin). 
-  move:a. 
-  cut:=eqEcard (fdom m) (frng m);rewrite leq_card_rng_dom/=. 
-  cut->//=:fdom m \subset frng m. 
-  + by move=> x; rewrite mem_fdom mem_frng hyp.
-  smt(mem_fdom mem_frng).
-  qed.
+  local module PInit (P : ODPRIMITIVE) : OPRIMITIVE = {
+    proc init () = {}
+    proc f  = P.f
+    proc fi = P.fi
+  }.
 
 
-  local equiv equiv_sponge_perm c m :
-      FInit(CSetSize(Sponge, Perm)).get ~ FInit(DFSetSize(FC(Sponge(Perm)))).get :
-    ={arg, glob Perm} /\ invm Perm.m{1} Perm.mi{1} /\ 
-      Cntr.c{2} = c /\ arg{2} = m /\
-      (Cntr.c + ((size arg + 1) %/ Common.r + 1) + 
-      max ((size_out + Common.r - 1) %/ Common.r - 1) 0 <= limit){2} ==>
-    ={res, glob Perm} /\ invm Perm.m{1} Perm.mi{1} /\ 
-      Cntr.c{2} = c + ((size m + 1) %/ Common.r + 1) + 
-      max ((size_out + Common.r - 1) %/ Common.r - 1) 0.
-  proof.
-  proc; inline FC(Sponge(Perm)).f; sp.
-  rcondt{2} 1; auto; sp.
-  call(: ={glob Perm} /\ invm Perm.m{1} Perm.mi{1})=>/=; auto; inline*.
-  while(={i, n, sa, sc, z, glob Perm} /\ invm Perm.m{1} Perm.mi{1}); auto.
-  + sp; if; auto; sp; if; auto; progress.
-    rewrite invm_set //=.
-    by move:H4; rewrite supp_dexcepted.
-  sp; conseq(:_==> ={i, n, sa, sc, glob Perm} /\ invm Perm.m{1} Perm.mi{1}); auto.
-  while(={xs, sa, sc, glob Perm} /\ invm Perm.m{1} Perm.mi{1}); auto.
-  sp; if; auto; progress. 
-  rewrite invm_set=>//=.
-  by move:H4; rewrite supp_dexcepted.
-  qed.
+local module OF (F : Oracle) : OIndif.ODFUNCTIONALITY = {
+  proc f = F.get
+}.
 
 
-  clone import Program as Prog2 with
-    type t <- bool,
-    op d <- dbool
-    proof *.
+local module Log = {
+  var m : (bool list * int, bool) fmap
+}.
 
-  local equiv equiv_ro_iro c m :
-    FInit(RO).get ~ FInit(DFSetSize(FC(BIRO.IRO))).get :
-    ={arg} /\ same_ro SRO.RO.RO.m{1} BIRO.IRO.mp{2} /\
-    arg{2} = m /\ Cntr.c{2} = c /\
-    (Cntr.c + ((size arg + 1) %/ Common.r + 1) + 
-      max ((size_out + Common.r - 1) %/ Common.r - 1) 0 <= limit){2}
-    ==> ={res} /\ same_ro SRO.RO.RO.m{1} BIRO.IRO.mp{2} /\ 
-      Cntr.c{2} = c + ((size m + 1) %/ Common.r + 1) + 
-      max ((size_out + Common.r - 1) %/ Common.r - 1) 0.
-  proof.
-  proc; inline *; sp; rcondt{2} 1; 1: auto.
-  swap{2} 1 5; sp; wp 2 1.
-  conseq(:_==> oget SRO.RO.RO.m{1}.[x{1}] = oget (of_list bs0{2}) /\
-    same_ro SRO.RO.RO.m{1} BIRO.IRO.mp{2}); 1:by auto.
-  rcondt{2} 1; 1: auto.
-  case: (x{1} \in SRO.RO.RO.m{1}).
-  + rcondf{1} 2; auto.
-    exists* BIRO.IRO.mp{2}; elim* => mp.
-    while{2}(bs0{2} = map (fun j => oget BIRO.IRO.mp{2}.[(x0{2},j)]) (range 0 i{2})
-        /\ n0{2} = size_out /\ x0{2} \in SRO.RO.RO.m{1} /\ 0 <= i{2} <= size_out
-        /\ same_ro SRO.RO.RO.m{1} BIRO.IRO.mp{2} /\ BIRO.IRO.mp{2} = mp)
-      (size_out - i{2}); auto.
-    - sp; rcondf 1; auto; 1: smt().
-      progress. 
-      * have/=<-:= map_rcons (fun (j : int) => oget BIRO.IRO.mp{hr}.[(x0{hr}, j)]) (range 0 i{hr}) i{hr}.
-        by rewrite !rangeSr //=.
-      * smt().
-      * smt().
-      * smt().
-    progress. 
-    - by rewrite range_geq.
-    - smt(size_out_gt0).
-    - smt().
-    - exact(dout_ll).
-    - have[] h[#] h1 h2 := H.
-      cut->:i_R = size_out by smt().
-      cut<-:=h2 _ H3.
-      smt(to_listK).
-  rcondt{1} 2; 1: auto; wp =>/=.
-  exists* BIRO.IRO.mp{2}; elim* => mp.
-  conseq(:_==> 
-        same_ro SRO.RO.RO.m{1} mp /\ i{2} = size_out /\
-        (forall (l,j),  (l,j) \in mp => (l,j) \in BIRO.IRO.mp{2}) /\
-        (forall (l,j),  (l,j) \in mp => BIRO.IRO.mp{2}.[(l,j)] = mp.[(l,j)]) /\
-        (forall (l,j), (l,j) \in BIRO.IRO.mp{2} => (l,j) \in mp \/ (l = x0{2} /\ 0 <= j < i{2})) /\
-        (forall j, 0 <= j < i{2} => (x0{2},j) \in BIRO.IRO.mp{2}) /\
-        take i{2} (to_list r{1}) = bs0{2} /\
-        take i{2} (to_list r{1}) = map (fun (j : int) => oget BIRO.IRO.mp{2}.[(x0{2}, j)]) (range 0 i{2})); progress=>//=.
-  + by rewrite get_set_sameE /= oget_some; smt(to_listK take_oversize spec_dout).
-  + move:H8; rewrite mem_set=>[][]//=h; 1:rewrite H3=>//=.
-    - by have []h1 []h2 h3:= H2; have->//:=h1 _ h.
-    by move:h => <<-; rewrite H6 //=.
-  + rewrite mem_set//=; have[]//=h:= H5 _ _ H11; left.
-    have []h1 []->//=:= H2.
-    by exists i0=>//=.
-  + move:H7; rewrite take_oversize 1:spec_dout//= => H7.
-    move:H10; rewrite mem_set. 
-    case(m \in SRO.RO.RO.m{1})=>//=h.
-    - rewrite get_set_neqE; 1:smt().
-      have []h1 []h2 ->//=:= H2. 
-      by apply eq_in_map=> j;rewrite mem_range=>[][]hj1 hj2/=; rewrite H4//=h1//=.
-    by move=><<-; rewrite get_set_eqE//=.
-  alias{1} 1 l = [<:bool>].
-  transitivity{1} {
-      l <@ Sample.sample(size_out);
-      r <- oget (of_list l);
+local module ExtendOutputSize (F : Oracle) : ODFUNCTIONALITY = {
+  proc f (x : bool list, k : int) = {
+    var o, l, suffix, prefix, i;
+    l <- None;
+    prefix <- [];
+    suffix <- [];
+    o <@ F.get(x);
+    prefix <- take k (to_list (oget o));
+    i <- size_out;
+    while (i < k) {
+      if ((x,i) \notin Log.m) {
+        Log.m.[(x,i)] <$ {0,1};
+      }
+      suffix <- rcons suffix (oget Log.m.[(x,i)]);
+      i <- i + 1;
     }
-    (={glob SRO.RO.RO, x} ==> ={glob SRO.RO.RO, r})
-    (x{1} = x0{2} /\ i{2} = 0 /\ n0{2} = size_out /\ mp = BIRO.IRO.mp{2} /\
-      same_ro SRO.RO.RO.m{1} BIRO.IRO.mp{2} /\ x{1} \notin SRO.RO.RO.m{1} /\
-      bs0{2} = []
-      ==>
-      same_ro SRO.RO.RO.m{1} mp /\ i{2} = size_out /\
-      (forall (l,j),  (l,j) \in mp => (l,j) \in BIRO.IRO.mp{2}) /\
-      (forall (l,j),  (l,j) \in mp => BIRO.IRO.mp{2}.[(l,j)] = mp.[(l,j)]) /\
-      (forall (l,j), (l,j) \in BIRO.IRO.mp{2} => (l,j) \in mp \/ (l = x0{2} /\ 0 <= j < i{2})) /\
-      (forall j, 0 <= j < i{2} => (x0{2},j) \in BIRO.IRO.mp{2}) /\
-      take i{2} (to_list r{1}) = bs0{2} /\
-      take i{2} (to_list r{1}) = 
-        map (fun (j : int) => oget BIRO.IRO.mp{2}.[(x0{2}, j)]) (range 0 i{2})); 
-    progress.
-  + smt().
-  + inline*; sp; wp. 
-    rnd to_list (fun x => oget (of_list x)); auto; progress. 
-    - smt(spec_dout supp_dlist to_listK spec2_dout size_out_gt0).
-    - rewrite -dout_equal_dlist dmap1E; apply mu_eq=> x/=. 
-      smt(to_listK).
-    - rewrite-dout_equal_dlist supp_dmap; smt(dout_full).
-    smt(to_listK).
-  wp=>/=.
-  conseq(:_==> i{2} = size_out /\ size l{1} = size_out /\
-      (forall (l0 : bool list) (j : int),
-        (l0, j) \in mp => (l0, j) \in BIRO.IRO.mp{2}) /\
-      (forall (l0 : bool list) (j : int),
-        (l0, j) \in mp => BIRO.IRO.mp{2}.[(l0, j)] = mp.[(l0, j)]) /\
-      (forall (l0 : bool list) (j : int),
-        (l0, j) \in BIRO.IRO.mp{2} => ((l0, j) \in mp) \/ (l0 = x0{2} /\ 0 <= j < i{2})) /\
-      (forall (j : int), 0 <= j < i{2} => (x0{2}, j) \in BIRO.IRO.mp{2}) /\
-      take i{2} l{1} = bs0{2} /\
-      take i{2} l{1} =
-        map (fun (j : int) => oget BIRO.IRO.mp{2}.[(x0{2}, j)]) (range 0 i{2}));
-    progress.
-  + have[]//=h h1:=to_listK (oget (of_list l_L)) l_L; rewrite h1//==> {h1 h}.
-    smt(spec2_dout).
-  + have[]//=h h1:=to_listK (oget (of_list l_L)) l_L; rewrite h1//==> {h1 h}.
-    smt(spec2_dout).
-  transitivity{1} {
-      l <@ LoopSnoc.sample(size_out);
-    }
-    (={glob SRO.RO.RO} ==> ={glob SRO.RO.RO, l})
-    (x{1} = x0{2} /\ i{2} = 0 /\ n0{2} = size_out /\ mp = BIRO.IRO.mp{2} /\
-      same_ro SRO.RO.RO.m{1} BIRO.IRO.mp{2} /\ x0{2} \notin SRO.RO.RO.m{1} /\
-      bs0{2} = []
-      ==>
-      i{2} = size_out /\ size l{1} = size_out /\
-      (forall (l,j),  (l,j) \in mp => (l,j) \in BIRO.IRO.mp{2}) /\
-      (forall (l,j),  (l,j) \in mp => BIRO.IRO.mp{2}.[(l,j)] = mp.[(l,j)]) /\
-      (forall (l,j), (l,j) \in BIRO.IRO.mp{2} => (l,j) \in mp \/ (l = x0{2} /\ 0 <= j < i{2})) /\
-      (forall j, 0 <= j < i{2} => (x0{2},j) \in BIRO.IRO.mp{2}) /\
-      take i{2} l{1} = bs0{2} /\
-      take i{2} l{1} = 
-        map (fun (j : int) => oget BIRO.IRO.mp{2}.[(x0{2}, j)]) (range 0 i{2})); 
-    progress.
-  + smt(). 
-  + by call Sample_LoopSnoc_eq; auto.
-  inline*; sp; wp.
-  conseq(:_==> i{2} = size_out /\ size l0{1} = i{2} /\ 
-      same_ro SRO.RO.RO.m{1} mp /\ x0{2} \notin SRO.RO.RO.m{1} /\
-      (forall l j, (l,j) \in mp => (l,j) \in BIRO.IRO.mp{2}) /\
-      (forall l j, (l,j) \in mp => BIRO.IRO.mp{2}.[(l, j)] = mp.[(l, j)]) /\
-      (forall l j, (l, j) \in BIRO.IRO.mp{2} => ((l, j) \in mp) \/ (l = x0{2} /\ 0 <= j < i{2})) /\
-      (forall j, 0 <= j < i{2} => (x0{2}, j) \in BIRO.IRO.mp{2}) /\
-      l0{1} = bs0{2} /\ bs0{2} = 
-        map (fun (j : int) => oget BIRO.IRO.mp{2}.[(x0{2}, j)]) (range 0 i{2})); progress.
-  + smt(take_oversize).
-  + smt(take_oversize).
-  while(0 <= i{2} <= size_out /\ size l0{1} = i{2} /\ n0{2} = size_out /\
-      ={i} /\ n{1} = n0{2} /\
-      same_ro SRO.RO.RO.m{1} mp /\ x0{2} \notin SRO.RO.RO.m{1} /\
-      (forall l j, (l,j) \in mp => (l,j) \in BIRO.IRO.mp{2}) /\
-      (forall l j, (l,j) \in mp => BIRO.IRO.mp{2}.[(l, j)] = mp.[(l, j)]) /\
-      (forall l j, (l, j) \in BIRO.IRO.mp{2} => ((l, j) \in mp) \/ (l = x0{2} /\ 0 <= j < i{2})) /\
-      (forall j, 0 <= j < i{2} => (x0{2}, j) \in BIRO.IRO.mp{2}) /\
-      l0{1} = bs0{2} /\ bs0{2} = 
-        map (fun (j : int) => oget BIRO.IRO.mp{2}.[(x0{2}, j)]) (range 0 i{2})).
-  + sp; wp=> //=.
-    rcondt{2} 1; 1:auto; progress.
-    - have[]h1 [] h2 h3 := H1.
-      have:=h2 x0{hr}; rewrite H2/= negb_exists/= =>/(_ (size bs0{hr})).
-      rewrite size_ge0 H9/=; apply absurd =>/= h.
-      by have //=:= H5 _ _ h.
-    rnd; auto; progress.
-    - smt(size_ge0).
-    - smt().
-    - by rewrite size_cat/=.
-    - by rewrite mem_set; left; rewrite H3. 
-    - rewrite get_setE (H4 _ _ H12).
-      cut/#: !(l1, j) = (x0{2}, size bs0{2}).
-      move:H2; apply absurd=> //=[#] <<- ->>.
-      have[] h1 [] h2 h3 := H1.
-      by apply h2; smt().
-    - move:H12; rewrite mem_set.
-      case((l1, j) \in BIRO.IRO.mp{2})=>//= h; 1: smt().
-      by move=> [#] <<- ->> //=; rewrite size_ge0; smt().
-    - rewrite mem_set.
-      case(j = size bs0{2})=>//=.
-      move=> h; rewrite h /=; have {H13} H13 {h} : j < size bs0{2} by smt().
-      by apply H6. 
-    - by rewrite cats1 get_set_sameE oget_some. 
-    - rewrite get_set_sameE oget_some H7 rangeSr.
-      rewrite !size_map 1:size_ge0. 
-      rewrite (size_map _ (range 0 (size bs0{2}))) size_range /=.
-      rewrite max_ler 1:size_ge0 map_rcons /=get_set_sameE oget_some; congr.
-      apply eq_in_map=> j.
-      rewrite mem_range /==> [] [] hj1 hj2.
-      by rewrite get_set_neqE //=; smt().
-  auto; progress.
-  + smt(size_out_gt0).
-  + smt().
-  + smt(). 
-  + by rewrite range_geq.
-  smt().
-  qed.
-
-  lemma Sponge_second_preimage_resistant &m mess :
-      (D2Pre.m2{m} = mess) =>
-      Pr[SRO.SecondPreimage(A, FM(CSetSize(Sponge), Perm)).main(mess) @ &m : res] <=
-      (limit ^ 2 - limit)%r / (2 ^ (r + c + 1))%r +
-      (4 * limit ^ 2)%r / (2 ^ c)%r +
-      (sigma + 1)%r / (2%r ^ size_out).
-  proof.  
-  move=> init_mess.
-  rewrite -(doutE1 witness).
-  rewrite(second_preimage_resistant_if_indifferentiable A A_ll (CSetSize(Sponge)) Perm &m mess init_mess).
-  exists (SimSetSize(Simulator)); split.
-  + by move=> F _; proc; inline*; auto.
-  cut->:Pr[Indiff0.Indif(CSetSize(Sponge, Perm), Perm, D2Pre(A)).main() @ &m : res] =
-        Pr[RealIndif(Sponge, Perm, DRestr(DSetSize(D2Pre(A)))).main() @ &m : res].
-  + byequiv=>//=; proc. 
-    inline Perm.init CSetSize(Sponge, Perm).init Sponge(Perm).init 
-          FC(Sponge(Perm)).init; sp.
-    inline D2Pre(A, CSetSize(Sponge, Perm), Perm).distinguish.
-    inline DRestr(DSetSize(D2Pre(A)), Sponge(Perm), Perm).distinguish 
-          DSetSize(D2Pre(A), FC(Sponge(Perm)), PC(Perm)).distinguish Cntr.init.
-    inline SRO.SecondPreimage(A, FInit(CSetSize(Sponge, Perm))).main
-        SRO.SecondPreimage(A, FInit(DFSetSize(FC(Sponge(Perm))))).main.
-    inline SRO.Bounder(FInit(CSetSize(Sponge, Perm))).init
-          SRO.Bounder(FInit(DFSetSize(FC(Sponge(Perm))))).init 
-          SRO.Counter.init FInit(DFSetSize(FC(Sponge(Perm)))).init
-          FInit(CSetSize(Sponge, Perm)).init.
-    wp; sp; sim. 
-    seq 1 1 : (={m1, m2, glob SRO.Counter, glob Perm}
-          /\ invm Perm.m{1} Perm.mi{1}
-          /\ ={c}(SRO.Counter,Cntr)); last first.
-    - if; auto; sp.
-      case(SRO.Counter.c{1} + ((size m2{1} + 1) %/ r + 1) + 
-          max ((size_out + r - 1) %/ r - 1) 0 < limit); last first.
-      * rcondf{1} 2; 1: by auto; inline*; auto; conseq(: _ ==> true); auto.
-        rcondf{2} 2; 1: by auto; inline*; auto; conseq(: _ ==> true); auto.
-        auto; inline*; auto; sp; conseq(: _ ==> true); auto.
-        if{2}; sp; auto; sim.
-        while{1}(invm Perm.m{1} Perm.mi{1}) (((size_out + r - 1) %/ r)-i{1}).
-        + auto; sp; if; auto. 
-          - sp; if ;auto; progress.
-            * exact (useful _ _ _ H H2).
-            * rewrite invm_set=>//=. 
-              by move:H4; rewrite  supp_dexcepted.
-            * smt().
-            smt().
-          smt().
-        conseq(:_==> invm Perm.m{1} Perm.mi{1}); 1:smt().
-        while{1}(invm Perm.m{1} Perm.mi{1})(size xs{1}).
-        + move=> _ z; auto; sp; if; auto; progress.
-          * exact (useful _ _ _ H H1).
-          * rewrite invm_set=>//=.
-            by move:H3; rewrite supp_dexcepted.
-          * smt().
-          smt().
-        auto; smt(size_ge0 size_eq0).
-      rcondt{1} 2; first by auto; inline*; auto; conseq(:_==> true); auto.
-      rcondt{2} 2; first by auto; inline*; auto; conseq(:_==> true); auto.
-      sim.
-      exists* m1{1}, m2{1}; elim* => a1 a2 c1 c2.
-      call (equiv_sponge_perm (c2 + ((size a1 + 1) %/ r + 1) + max ((size_out + r - 1) %/ r - 1) 0) a2).
-      auto; call (equiv_sponge_perm c2 a1); auto; progress. 
-      smt(List.size_ge0 divz_ge0 gt0_r).
-      smt(List.size_ge0 divz_ge0 gt0_r).
-    call(: ={glob SRO.Counter, glob Perm, glob SRO.Bounder}
-          /\ invm Perm.m{1} Perm.mi{1} /\ ={c}(SRO.Counter,Cntr)).
-    + proc; sp; if; auto; sp; if; auto; sp.
-      exists * x{1}; elim* => m c1 c2 b1 b2.
-      by call(equiv_sponge_perm c1 m); auto; smt().
-    inline*; auto; progress.
-    by rewrite /invm=> x y; rewrite 2!emptyE.
-  cut->:Pr[Indiff0.Indif(RO, SimSetSize(Simulator, RO), D2Pre(A)).main() @ &m : res] =
-        Pr[IdealIndif(BIRO.IRO, Simulator, DRestr(DSetSize(D2Pre(A)))).main() @ &m : res].
-  + byequiv=>//=; proc.
-    inline Simulator(FGetSize(RO)).init RO.init Simulator(BIRO.IRO).init 
-          BIRO.IRO.init Gconcl_list.BIRO2.IRO.init; sp.
-    inline D2Pre(A, RO, Simulator(FGetSize(RO))).distinguish.
-    inline DRestr(DSetSize(D2Pre(A)), BIRO.IRO, Simulator(BIRO.IRO)).distinguish 
-          DSetSize(D2Pre(A), FC(BIRO.IRO), PC(Simulator(BIRO.IRO))).distinguish; wp; sim.
-    inline SRO.Bounder(FInit(DFSetSize(FC(BIRO.IRO)))).init 
-          SRO.Bounder(FInit(RO)).init SRO.Counter.init FInit(RO).init
-          FInit(DFSetSize(FC(BIRO.IRO))).init Cntr.init; sp.
-    inline SRO.SecondPreimage(A, FInit(RO)).main 
-          SRO.SecondPreimage(A, FInit(DFSetSize(FC(BIRO.IRO)))).main.
-    inline SRO.Bounder(FInit(RO)).init 
-          SRO.Bounder(FInit(DFSetSize(FC(BIRO.IRO)))).init SRO.Counter.init
-          FInit(RO).init FInit(DFSetSize(FC(BIRO.IRO))).init.
-    sp; sim.
-    seq 1 1 : (={m1, m2, glob SRO.Counter}
-          /\ ={c}(SRO.Counter,Cntr)
-          /\ same_ro SRO.RO.RO.m{1} BIRO.IRO.mp{2}); last first.
-    - if; auto; sp.
-      case: (SRO.Counter.c{1} + ((size m2{1} + 1) %/ r + 1) + 
-          max ((size_out + r - 1) %/ r - 1) 0 < limit); last first. 
-      * rcondf{1} 2; first by auto; inline*; auto.
-        rcondf{2} 2; first auto; inline*; auto; sp.
-        + rcondt 1; first by auto; smt().
-          by sp; rcondt 1; auto; conseq(:_==> true); auto.
-        inline*;sp; auto.
-        rcondt{2} 1; first by auto; smt().
-        conseq(:_==> true); first smt(dout_ll).
-        sp; rcondt{2} 1; auto; conseq(:_==> true); auto.
-        by while{2}(true)(n0{2}-i{2}); auto; 1:(sp; if; auto); smt(dbool_ll).
-      rcondt{1} 2; first by auto; inline*; auto.
-      rcondt{2} 2; first auto; inline*; auto; sp.
-      + rcondt 1; first by auto; smt().
-        by sp; rcondt 1; auto; conseq(:_==> true); auto.
-      sim.
-      exists* m1{1}, m2{1}; elim*=> a1 a2 c1 c2.
-      call(equiv_ro_iro (c2 + ((size a1 + 1) %/ r + 1) + 
-          max ((size_out + r - 1) %/ r - 1) 0) a2).
-      auto; call(equiv_ro_iro c2 a1); auto; smt().
-    call(: ={glob SRO.Counter, glob SRO.Bounder} /\ ={c}(SRO.Counter,Cntr)
-          /\ same_ro SRO.RO.RO.m{1} BIRO.IRO.mp{2}); auto.
-    + proc; sp; if; auto; sp; if; auto; sp.
-      exists* x{1}; elim* => a c1 c2 b1 b2.
-      call(equiv_ro_iro c1 a); auto; smt().
-    smt(mem_empty). 
-  have->//=:= SHA3Indiff (DSetSize(D2Pre(A))) &m _.
-  move=> F P P_f_ll P_fi_ll F_ll; proc; inline*; auto; sp.
-  seq 1 : true; auto.
-  + call (A_ll (SRO.Bounder(FInit(DFSetSize(F))))); auto.
-    by proc; inline*; sp; if; auto; sp; if; auto; sp; call F_ll; auto.
-  if; auto; sp.
-  seq 1 : true; auto.
-  + by call F_ll; auto.
-  sp; if; auto; sp; call F_ll; auto.
-  qed.
-
-end section SecondPreimage.
-
-
-
-section Collision.
-
-  declare module A : SRO.AdvCollision{SRO.RO.RO, SRO.RO.FRO, SRO.Bounder, Perm, 
-    Gconcl_list.BIRO2.IRO, Simulator, Cntr, BIRO.IRO, F.RO, F.FRO, Redo, C, 
-    Gconcl.S, BlockSponge.BIRO.IRO, BlockSponge.C, Gconcl_list.F2.RO,
-    Gconcl_list.F2.FRO, Gconcl_list.Simulator}.
-
-  axiom A_ll (F <: SRO.Oracle) : islossless F.get => islossless A(F).guess.
-
-  local lemma invm_dom_rng (m mi : (state, state) fmap) :
-      invm m mi => dom m = rng mi.
-  proof. 
-  move=>h; rewrite fun_ext=> x; rewrite domE rngE /= eq_iff; have h2 := h x; split.
-  + move=> m_x_not_None; exists (oget m.[x]); rewrite -h2; move: m_x_not_None.
-    by case: (m.[x]).
-  by move=> [] a; rewrite -h2 => ->.
-  qed.
-
-  local lemma invmC' (m mi : (state, state) fmap) :
-      invm m mi => invm mi m.
-  proof. by rewrite /#. qed.
-
-  local lemma invmC (m mi : (state, state) fmap) :
-      invm m mi <=> invm mi m.
-  proof. by split;exact invmC'. qed.
-
-  local lemma useful m mi a :
-      invm m mi => ! a \in m => Distr.is_lossless ((bdistr `*` cdistr) \ rng m).
-  proof.
-  move=>hinvm nin_dom.
-  cut prod_ll:Distr.is_lossless (bdistr `*` cdistr).
-  + by rewrite dprod_ll DBlock.dunifin_ll DCapacity.dunifin_ll. 
-  apply dexcepted_ll=>//=;rewrite-prod_ll.
-  cut->:predT = predU (predC (rng m)) (rng m);1:rewrite predCU//=.
-  rewrite Distr.mu_disjoint 1:predCI//=StdRing.RField.addrC. 
-  cut/=->:=StdOrder.RealOrder.ltr_add2l (mu (bdistr `*` cdistr) (rng m)) 0%r.
-  rewrite Distr.witness_support/predC.
-  move:nin_dom;apply absurd=>//=;rewrite negb_exists/==>hyp. 
-  cut{hyp}hyp:forall x, rng m x by smt(supp_dprod DBlock.supp_dunifin DCapacity.supp_dunifin). 
-  move:a. 
-  cut:=eqEcard (fdom m) (frng m);rewrite leq_card_rng_dom/=. 
-  cut->//=:fdom m \subset frng m. 
-  + by move=> x; rewrite mem_fdom mem_frng hyp.
-  smt(mem_fdom mem_frng).
-  qed.
-
-
-  local equiv equiv_sponge_perm c m :
-      FInit(CSetSize(Sponge, Perm)).get ~ FInit(DFSetSize(FC(Sponge(Perm)))).get :
-    ={arg, glob Perm} /\ invm Perm.m{1} Perm.mi{1} /\ 
-      Cntr.c{2} = c /\ arg{2} = m /\
-      (Cntr.c + ((size arg + 1) %/ Common.r + 1) + 
-      max ((size_out + Common.r - 1) %/ Common.r - 1) 0 <= limit){2} ==>
-    ={res, glob Perm} /\ invm Perm.m{1} Perm.mi{1} /\ 
-      Cntr.c{2} = c + ((size m + 1) %/ Common.r + 1) + 
-      max ((size_out + Common.r - 1) %/ Common.r - 1) 0.
-  proof.
-  proc; inline FC(Sponge(Perm)).f; sp.
-  rcondt{2} 1; auto; sp.
-  call(: ={glob Perm} /\ invm Perm.m{1} Perm.mi{1})=>/=; auto; inline*.
-  while(={i, n, sa, sc, z, glob Perm} /\ invm Perm.m{1} Perm.mi{1}); auto.
-  + sp; if; auto; sp; if; auto; progress.
-    rewrite invm_set //=.
-    by move:H4; rewrite supp_dexcepted.
-  sp; conseq(:_==> ={i, n, sa, sc, glob Perm} /\ invm Perm.m{1} Perm.mi{1}); auto.
-  while(={xs, sa, sc, glob Perm} /\ invm Perm.m{1} Perm.mi{1}); auto.
-  sp; if; auto; progress. 
-  rewrite invm_set=>//=.
-  by move:H4; rewrite supp_dexcepted.
-  qed.
-
-  clone import Program as Prog3 with
-    type t <- bool,
-    op d <- dbool
-    proof *.
-
-  local equiv equiv_ro_iro c m :
-    FInit(RO).get ~ FInit(DFSetSize(FC(BIRO.IRO))).get :
-    ={arg} /\ same_ro SRO.RO.RO.m{1} BIRO.IRO.mp{2} /\
-    arg{2} = m /\ Cntr.c{2} = c /\
-    (Cntr.c + ((size arg + 1) %/ Common.r + 1) + 
-      max ((size_out + Common.r - 1) %/ Common.r - 1) 0 <= limit){2}
-    ==> ={res} /\ same_ro SRO.RO.RO.m{1} BIRO.IRO.mp{2} /\ 
-      Cntr.c{2} = c + ((size m + 1) %/ Common.r + 1) + 
-      max ((size_out + Common.r - 1) %/ Common.r - 1) 0.
-  proof.
-  proc; inline *; sp; rcondt{2} 1; 1: auto.
-  swap{2} 1 5; sp; wp 2 1.
-  conseq(:_==> oget SRO.RO.RO.m{1}.[x{1}] = oget (of_list bs0{2}) /\
-    same_ro SRO.RO.RO.m{1} BIRO.IRO.mp{2}); 1:by auto.
-  rcondt{2} 1; 1: auto.
-  case: (x{1} \in SRO.RO.RO.m{1}).
-  + rcondf{1} 2; auto.
-    exists* BIRO.IRO.mp{2}; elim* => mp.
-    while{2}(bs0{2} = map (fun j => oget BIRO.IRO.mp{2}.[(x0{2},j)]) (range 0 i{2})
-        /\ n0{2} = size_out /\ x0{2} \in SRO.RO.RO.m{1} /\ 0 <= i{2} <= size_out
-        /\ same_ro SRO.RO.RO.m{1} BIRO.IRO.mp{2} /\ BIRO.IRO.mp{2} = mp)
-      (size_out - i{2}); auto.
-    - sp; rcondf 1; auto; 1: smt().
-      progress. 
-      * have/=<-:= map_rcons (fun (j : int) => oget BIRO.IRO.mp{hr}.[(x0{hr}, j)]) (range 0 i{hr}) i{hr}.
-        by rewrite !rangeSr //=.
-      * smt().
-      * smt().
-      * smt().
-    progress. 
-    - by rewrite range_geq.
-    - smt(size_out_gt0).
-    - smt().
-    - exact(dout_ll).
-    - have[] h[#] h1 h2 := H.
-      cut->:i_R = size_out by smt().
-      cut<-:=h2 _ H3.
-      smt(to_listK).
-  rcondt{1} 2; 1: auto; wp =>/=.
-  exists* BIRO.IRO.mp{2}; elim* => mp.
-  conseq(:_==> 
-        same_ro SRO.RO.RO.m{1} mp /\ i{2} = size_out /\
-        (forall (l,j),  (l,j) \in mp => (l,j) \in BIRO.IRO.mp{2}) /\
-        (forall (l,j),  (l,j) \in mp => BIRO.IRO.mp{2}.[(l,j)] = mp.[(l,j)]) /\
-        (forall (l,j), (l,j) \in BIRO.IRO.mp{2} => (l,j) \in mp \/ (l = x0{2} /\ 0 <= j < i{2})) /\
-        (forall j, 0 <= j < i{2} => (x0{2},j) \in BIRO.IRO.mp{2}) /\
-        take i{2} (to_list r{1}) = bs0{2} /\
-        take i{2} (to_list r{1}) = map (fun (j : int) => oget BIRO.IRO.mp{2}.[(x0{2}, j)]) (range 0 i{2})); progress=>//=.
-  + by rewrite get_set_sameE /= oget_some; smt(to_listK take_oversize spec_dout).
-  + move:H8; rewrite mem_set=>[][]//=h; 1:rewrite H3=>//=.
-    - by have []h1 []h2 h3:= H2; have->//:=h1 _ h.
-    by move:h => <<-; rewrite H6 //=.
-  + rewrite mem_set //=; have [] //= h:= H5 _ _ H11; left.
-    have []h1 []->//=:= H2.
-    by exists i0=>//=.
-  + move:H7; rewrite take_oversize 1:spec_dout//= => H7.
-    move:H10; rewrite mem_set. 
-    case(m \in SRO.RO.RO.m{1})=>//=h.
-    - rewrite get_set_neqE; 1:smt().
-      have []h1 []h2 ->//=:= H2. 
-      by apply eq_in_map=> j;rewrite mem_range=>[][]hj1 hj2/=; rewrite H4//=h1//=.
-    by move=><<-; rewrite get_set_eqE//=.
-  alias{1} 1 l = [<:bool>].
-  transitivity{1} {
-      l <@ Sample.sample(size_out);
-      r <- oget (of_list l);
-    }
-    (={glob SRO.RO.RO, x} ==> ={glob SRO.RO.RO, r})
-    (x{1} = x0{2} /\ i{2} = 0 /\ n0{2} = size_out /\ mp = BIRO.IRO.mp{2} /\
-      same_ro SRO.RO.RO.m{1} BIRO.IRO.mp{2} /\ x{1} \notin SRO.RO.RO.m{1} /\
-      bs0{2} = []
-      ==>
-      same_ro SRO.RO.RO.m{1} mp /\ i{2} = size_out /\
-      (forall (l,j),  (l,j) \in mp => (l,j) \in BIRO.IRO.mp{2}) /\
-      (forall (l,j),  (l,j) \in mp => BIRO.IRO.mp{2}.[(l,j)] = mp.[(l,j)]) /\
-      (forall (l,j), (l,j) \in BIRO.IRO.mp{2} => (l,j) \in mp \/ (l = x0{2} /\ 0 <= j < i{2})) /\
-      (forall j, 0 <= j < i{2} => (x0{2},j) \in BIRO.IRO.mp{2}) /\
-      take i{2} (to_list r{1}) = bs0{2} /\
-      take i{2} (to_list r{1}) = 
-        map (fun (j : int) => oget BIRO.IRO.mp{2}.[(x0{2}, j)]) (range 0 i{2})); 
-    progress.
-  + smt().
-  + inline*; sp; wp. 
-    rnd to_list (fun x => oget (of_list x)); auto; progress. 
-    - smt(spec_dout supp_dlist to_listK spec2_dout size_out_gt0). 
-    - rewrite -dout_equal_dlist dmap1E; apply mu_eq=> x/=. 
-      smt(to_listK).
-    - rewrite-dout_equal_dlist supp_dmap; smt(dout_full).
-    smt(to_listK).
-  wp=>/=.
-  conseq(:_==> i{2} = size_out /\ size l{1} = size_out /\
-      (forall (l0 : bool list) (j : int),
-        (l0, j) \in mp => (l0, j) \in BIRO.IRO.mp{2}) /\
-      (forall (l0 : bool list) (j : int),
-        (l0, j) \in mp => BIRO.IRO.mp{2}.[(l0, j)] = mp.[(l0, j)]) /\
-      (forall (l0 : bool list) (j : int),
-        (l0, j) \in BIRO.IRO.mp{2} => ((l0, j) \in mp) \/ (l0 = x0{2} /\ 0 <= j < i{2})) /\
-      (forall (j : int), 0 <= j < i{2} => (x0{2}, j) \in BIRO.IRO.mp{2}) /\
-      take i{2} l{1} = bs0{2} /\
-      take i{2} l{1} =
-        map (fun (j : int) => oget BIRO.IRO.mp{2}.[(x0{2}, j)]) (range 0 i{2}));
-    progress.
-  + have[]//=h h1:=to_listK (oget (of_list l_L)) l_L; rewrite h1//==> {h1 h}.
-    smt(spec2_dout).
-  + have[]//=h h1:=to_listK (oget (of_list l_L)) l_L; rewrite h1//==> {h1 h}.
-    smt(spec2_dout). 
-  transitivity{1} {
-      l <@ LoopSnoc.sample(size_out);
-    }
-    (={glob SRO.RO.RO} ==> ={glob SRO.RO.RO, l})
-    (x{1} = x0{2} /\ i{2} = 0 /\ n0{2} = size_out /\ mp = BIRO.IRO.mp{2} /\
-      same_ro SRO.RO.RO.m{1} BIRO.IRO.mp{2} /\ x0{2} \notin SRO.RO.RO.m{1} /\
-      bs0{2} = []
-      ==>
-      i{2} = size_out /\ size l{1} = size_out /\
-      (forall (l,j),  (l,j) \in mp => (l,j) \in BIRO.IRO.mp{2}) /\
-      (forall (l,j),  (l,j) \in mp => BIRO.IRO.mp{2}.[(l,j)] = mp.[(l,j)]) /\
-      (forall (l,j), (l,j) \in BIRO.IRO.mp{2} => (l,j) \in mp \/ (l = x0{2} /\ 0 <= j < i{2})) /\
-      (forall j, 0 <= j < i{2} => (x0{2},j) \in BIRO.IRO.mp{2}) /\
-      take i{2} l{1} = bs0{2} /\
-      take i{2} l{1} = 
-        map (fun (j : int) => oget BIRO.IRO.mp{2}.[(x0{2}, j)]) (range 0 i{2})); 
-    progress.
-  + smt(). 
-  + by call Sample_LoopSnoc_eq; auto.
-  inline*; sp; wp.
-  conseq(:_==> i{2} = size_out /\ size l0{1} = i{2} /\ 
-      same_ro SRO.RO.RO.m{1} mp /\ x0{2} \notin SRO.RO.RO.m{1} /\
-      (forall l j, (l,j) \in mp => (l,j) \in BIRO.IRO.mp{2}) /\
-      (forall l j, (l,j) \in mp => BIRO.IRO.mp{2}.[(l, j)] = mp.[(l, j)]) /\
-      (forall l j, (l, j) \in BIRO.IRO.mp{2} => ((l, j) \in mp) \/ (l = x0{2} /\ 0 <= j < i{2})) /\
-      (forall j, 0 <= j < i{2} => (x0{2}, j) \in BIRO.IRO.mp{2}) /\
-      l0{1} = bs0{2} /\ bs0{2} = 
-        map (fun (j : int) => oget BIRO.IRO.mp{2}.[(x0{2}, j)]) (range 0 i{2})); progress.
-  + smt(take_oversize).
-  + smt(take_oversize).
-  while(0 <= i{2} <= size_out /\ size l0{1} = i{2} /\ n0{2} = size_out /\
-      ={i} /\ n{1} = n0{2} /\
-      same_ro SRO.RO.RO.m{1} mp /\ x0{2} \notin SRO.RO.RO.m{1} /\
-      (forall l j, (l,j) \in mp => (l,j) \in BIRO.IRO.mp{2}) /\
-      (forall l j, (l,j) \in mp => BIRO.IRO.mp{2}.[(l, j)] = mp.[(l, j)]) /\
-      (forall l j, (l, j) \in BIRO.IRO.mp{2} => ((l, j) \in mp) \/ (l = x0{2} /\ 0 <= j < i{2})) /\
-      (forall j, 0 <= j < i{2} => (x0{2}, j) \in BIRO.IRO.mp{2}) /\
-      l0{1} = bs0{2} /\ bs0{2} = 
-        map (fun (j : int) => oget BIRO.IRO.mp{2}.[(x0{2}, j)]) (range 0 i{2})).
-  + sp; wp=> //=.
-    rcondt{2} 1; 1:auto; progress.
-    - have[]h1 [] h2 h3 := H1.
-      have:=h2 x0{hr}; rewrite H2/= negb_exists/= =>/(_ (size bs0{hr})).
-      rewrite size_ge0 H9/=; apply absurd =>/= h.
-      by have //=:= H5 _ _ h.
-    rnd; auto; progress.
-    - smt(size_ge0).
-    - smt().
-    - by rewrite size_cat/=.
-    - by rewrite mem_set; left; rewrite H3. 
-    - rewrite get_setE (H4 _ _ H12).
-      cut/#: !(l1, j) = (x0{2}, size bs0{2}).
-      move:H2; apply absurd=> //=[#] <<- ->>.
-      have[] h1 [] h2 h3 := H1.
-      by apply h2; smt().
-    - move:H12; rewrite mem_set.
-      case((l1, j) \in BIRO.IRO.mp{2})=>//= h; 1: smt().
-      by move=> [#] <<- ->> //=; rewrite size_ge0; smt().
-    - rewrite mem_set.
-      case(j = size bs0{2})=>//=.
-      move=> h; rewrite h /=; have {H13} H13 {h} : j < size bs0{2} by smt().
-      by apply H6. 
-    - by rewrite cats1 get_set_sameE oget_some. 
-    - rewrite get_set_sameE oget_some H7 rangeSr.
-      rewrite !size_map 1:size_ge0. 
-      rewrite (size_map _ (range 0 (size bs0{2}))) size_range /=.
-      rewrite max_ler 1:size_ge0 map_rcons /=get_set_sameE oget_some; congr.
-      apply eq_in_map=> j.
-      rewrite mem_range /==> [] [] hj1 hj2.
-      by rewrite get_set_neqE //=; smt().
-  auto; progress.
-  + smt(size_out_gt0).
-  + smt().
-  + smt(). 
-  + by rewrite range_geq.
-  smt().
-  qed.
-
-  lemma Sponge_coll_resistant &m :
-      Pr[SRO.Collision(A, FM(CSetSize(Sponge), Perm)).main() @ &m : res] <=
-      (limit ^ 2 - limit)%r / (2 ^ (r + c + 1))%r +
-      (4 * limit ^ 2)%r / (2 ^ c)%r +
-      (sigma * (sigma - 1) + 2)%r / 2%r / (2%r ^ size_out).
-  proof. 
-  rewrite -(doutE1 witness).
-  rewrite (coll_resistant_if_indifferentiable A A_ll (CSetSize(Sponge)) Perm &m).
-  exists (SimSetSize(Simulator)); split.
-  + by move=> F _; proc; inline*; auto.
-  cut->:Pr[Indiff0.Indif(CSetSize(Sponge, Perm), Perm, DColl(A)).main() @ &m : res] =
-        Pr[RealIndif(Sponge, Perm, DRestr(DSetSize(DColl(A)))).main() @ &m : res].
-  + byequiv=>//=; proc. 
-    inline Perm.init CSetSize(Sponge, Perm).init Sponge(Perm).init 
-          FC(Sponge(Perm)).init; sp.
-    inline DColl(A, CSetSize(Sponge, Perm), Perm).distinguish.
-    inline DRestr(DSetSize(DColl(A)), Sponge(Perm), Perm).distinguish 
-          DSetSize(DColl(A), FC(Sponge(Perm)), PC(Perm)).distinguish Cntr.init; wp; sp; sim. 
-    seq 2 2 : (={m1, m2, glob SRO.Counter, glob Perm}
-          /\ invm Perm.m{1} Perm.mi{1}
-          /\ ={c}(SRO.Counter,Cntr)); last first.
-    - if; auto; sp.
-      case(SRO.Counter.c{1} + ((size m2{1} + 1) %/ r + 1) + 
-          max ((size_out + r - 1) %/ r - 1) 0 < limit); last first.
-      * rcondf{1} 2; 1: by auto; inline*; auto; conseq(: _ ==> true); auto.
-        rcondf{2} 2; 1: by auto; inline*; auto; conseq(: _ ==> true); auto.
-        auto; inline*; auto; sp; conseq(: _ ==> true); auto.
-        if{2}; sp; auto; sim.
-        while{1}(invm Perm.m{1} Perm.mi{1}) (((size_out + r - 1) %/ r)-i{1}).
-        + auto; sp; if; auto. 
-          - sp; if ;auto; progress.
-            * exact (useful _ _ _ H H2).
-            * rewrite invm_set=>//=. 
-              by move:H4; rewrite  supp_dexcepted.
-            * smt().
-            smt().
-          smt().
-        conseq(:_==> invm Perm.m{1} Perm.mi{1}); 1:smt().
-        while{1}(invm Perm.m{1} Perm.mi{1})(size xs{1}).
-        + move=> _ z; auto; sp; if; auto; progress.
-          * exact (useful _ _ _ H H1).
-          * rewrite invm_set=>//=.
-            by move:H3; rewrite supp_dexcepted.
-          * smt().
-          smt().
-        auto; smt(size_ge0 size_eq0).
-      rcondt{1} 2; first by auto; inline*; auto; conseq(:_==> true); auto.
-      rcondt{2} 2; first by auto; inline*; auto; conseq(:_==> true); auto.
-      sim.
-      exists* m1{1}, m2{1}; elim* => a1 a2 c1 c2.
-      call (equiv_sponge_perm (c2 + ((size a1 + 1) %/ r + 1) + max ((size_out + r - 1) %/ r - 1) 0) a2).
-      auto; call (equiv_sponge_perm c2 a1); auto; progress. 
-      smt(List.size_ge0 divz_ge0 gt0_r).
-      smt(List.size_ge0 divz_ge0 gt0_r).
-    call(: ={glob SRO.Counter, glob Perm, glob SRO.Bounder}
-          /\ invm Perm.m{1} Perm.mi{1} /\ ={c}(SRO.Counter,Cntr)).
-    + proc; sp; if; auto; sp; if; auto; sp.
-      exists * x{1}; elim* => m c1 c2 b1 b2.
-      by call(equiv_sponge_perm c1 m); auto; smt().
-    inline*; auto; progress.
-    by rewrite /invm=> x y; rewrite 2!emptyE.
-  cut->:Pr[Indiff0.Indif(RO, SimSetSize(Simulator, RO), DColl(A)).main() @ &m : res] =
-        Pr[IdealIndif(BIRO.IRO, Simulator, DRestr(DSetSize(DColl(A)))).main() @ &m : res].
-  + byequiv=>//=; proc.
-    inline Simulator(FGetSize(RO)).init RO.init Simulator(BIRO.IRO).init 
-          BIRO.IRO.init Gconcl_list.BIRO2.IRO.init; sp.
-    inline DColl(A, RO, Simulator(FGetSize(RO))).distinguish.
-    inline DRestr(DSetSize(DColl(A)), BIRO.IRO, Simulator(BIRO.IRO)).distinguish 
-          DSetSize(DColl(A), FC(BIRO.IRO), PC(Simulator(BIRO.IRO))).distinguish; wp; sim.
-    inline SRO.Bounder(FInit(DFSetSize(FC(BIRO.IRO)))).init 
-          SRO.Bounder(FInit(RO)).init SRO.Counter.init FInit(RO).init
-          FInit(DFSetSize(FC(BIRO.IRO))).init Cntr.init; sp.
-    seq 1 1 : (={m1, m2, glob SRO.Counter}
-          /\ ={c}(SRO.Counter,Cntr)
-          /\ same_ro SRO.RO.RO.m{1} BIRO.IRO.mp{2}); last first.
-    - if; auto; sp.
-      case: (SRO.Counter.c{1} + ((size m2{1} + 1) %/ r + 1) + 
-          max ((size_out + r - 1) %/ r - 1) 0 < limit); last first. 
-      * rcondf{1} 2; first by auto; inline*; auto.
-        rcondf{2} 2; first auto; inline*; auto; sp.
-        + rcondt 1; first by auto; smt().
-          by sp; rcondt 1; auto; conseq(:_==> true); auto.
-        inline*;sp; auto.
-        rcondt{2} 1; first by auto; smt().
-        conseq(:_==> true); first smt(dout_ll).
-        sp; rcondt{2} 1; auto; conseq(:_==> true); auto.
-        by while{2}(true)(n0{2}-i{2}); auto; 1:(sp; if; auto); smt(dbool_ll).
-      rcondt{1} 2; first by auto; inline*; auto.
-      rcondt{2} 2; first auto; inline*; auto; sp.
-      + rcondt 1; first by auto; smt().
-        by sp; rcondt 1; auto; conseq(:_==> true); auto.
-      sim.
-      exists* m1{1}, m2{1}; elim*=> a1 a2 c1 c2.
-      call(equiv_ro_iro (c2 + ((size a1 + 1) %/ r + 1) + 
-          max ((size_out + r - 1) %/ r - 1) 0) a2).
-      auto; call(equiv_ro_iro c2 a1); auto; smt().
-    call(: ={glob SRO.Counter, glob SRO.Bounder} /\ ={c}(SRO.Counter,Cntr)
-          /\ same_ro SRO.RO.RO.m{1} BIRO.IRO.mp{2}); auto.
-    + proc; sp; if; auto; sp; if; auto; sp.
-      exists* x{1}; elim* => a c1 c2 b1 b2.
-      call(equiv_ro_iro c1 a); auto; smt().
-    smt(mem_empty). 
-  have->//=:= SHA3Indiff (DSetSize(DColl(A))) &m _.
-  move=> F P P_f_ll P_fi_ll F_ll; proc; inline*; auto; sp.
-  seq 1 : true; auto.
-  + call (A_ll (SRO.Bounder(FInit(DFSetSize(F))))); auto.
-    by proc; inline*; sp; if; auto; sp; if; auto; sp; call F_ll; auto.
-  if; auto; sp.
-  seq 1 : true; auto.
-  + by call F_ll; auto.
-  sp; if; auto; sp; call F_ll; auto.
-  qed.
-
-end section Collision.
-
-module X (F : SRO.Oracle) = {
-  proc get (bl : bool list) = {
-  var r;
-  r <@ F.get(bl ++ [ false ; true ]);
-  return r;
+    l <- Some (prefix ++ suffix);
+    return l;
   }
 }.
 
-module AdvCollisionSHA3 (A : SRO.AdvCollision) (F : SRO.Oracle) = {
-  proc guess () = {
-    var m1, m2;
-    (m1, m2) <@ A(X(F)).guess();
-    return (m1 ++ [ false ; true ], m2 ++ [ false ; true ]);
+local module OFC2 (F : Oracle) = OFC(ExtendOutputSize(F)).
+
+local module ExtendOutput (F : RF) = {
+  proc init () = {
+    Log.m <- empty;
+    F.init();
+  }
+  proc f = ExtendOutputSize(F).f
+  proc get = f
+}.
+
+  local module (Dist_of_P2Adv (A : SH.AdvSecondPreimage) : ODISTINGUISHER) (F : ODFUNCTIONALITY) (P : ODPRIMITIVE) = {
+    var m : bool list
+    proc distinguish () = {
+      var hash, hash', m';
+      Log.m <- empty;
+      m' <@ A(DFSetSize(F),P).guess(m);
+      hash  <@ DFSetSize(F).f(m);
+      hash' <@ DFSetSize(F).f(m');
+      return m <> m' /\ exists y, hash' = Some y /\ hash = Some y;
+    }
+  }.
+  
+
+local module (SORO_P2 (A : SH.AdvSecondPreimage) : SORO.AdvSecondPreimage) (F : Oracle) = {
+  proc guess (m : bool list) : bool list = {
+    var mi;
+    Log.m <- empty;
+    Counter.c <- 0;
+    Dist_of_P2Adv.m <- m;
+    OSimulator(ExtendOutputSize(F)).init();
+    mi <@ A(DFSetSize(OFC2(F)),OPC(OSimulator(ExtendOutputSize(F)))).guess(m);
+    return mi;
   }
 }.
 
-section SHA3_Collision.
+local module RFList = {
+  var m : (bool list, f_out) fmap
+  proc init () = {
+    m <- empty;
+  }
+  proc get (x : bool list) : f_out option = {
+    var z;
+    if (x \notin m) {
+      z <$ dlist dbool size_out;
+      m.[x] <- oget (of_list z);
+    }
+    return m.[x];
+  }
+  proc sample (x: bool list) = {}
+}.
 
-  declare module A : SRO.AdvCollision{SRO.RO.RO, SRO.RO.FRO, SRO.Bounder, Perm, 
-    Gconcl_list.BIRO2.IRO, Simulator, Cntr, BIRO.IRO, F.RO, F.FRO, Redo, C, 
-    Gconcl.S, BlockSponge.BIRO.IRO, BlockSponge.C, Gconcl_list.F2.RO,
-    Gconcl_list.F2.FRO, Gconcl_list.Simulator}.
+local module RFWhile = {
+  proc init () = {
+    RFList.m <- empty;
+  }
+  proc get (x : bool list) : f_out option = {
+    var l, i, b;
+    if (x \notin RFList.m) {
+      i <- 0;
+      l <- [];
+      while (i < size_out) {
+        b <$ dbool;
+        l <- rcons l b;
+        i <- i + 1;
+      }
+      RFList.m.[x] <- oget (of_list l);
+    }
+    return RFList.m.[x];
+  }
+  proc sample (x: bool list) = {}
+}.
 
-  axiom A_ll (F <: SRO.Oracle) : islossless F.get => islossless A(F).guess.
 
-  lemma SHA3_coll_resistant &m :
-      Pr[SRO.Collision(AdvCollisionSHA3(A), FM(CSetSize(Sponge), Perm)).main() @ &m : res] <=
-      (limit ^ 2 - limit)%r / (2 ^ (r + c + 1))%r +
-      (4 * limit ^ 2)%r / (2 ^ c)%r +
-      (sigma * (sigma - 1) + 2)%r / 2%r / (2%r ^ size_out).
+local equiv rw_RF_List_While :
+    RFList.get ~ RFWhile.get : 
+    ={arg, glob RFList} ==> ={res, glob RFWhile}.
+proof.
+proc; if; 1, 3: auto; wp.
+conseq(:_==> z{1} = l{2})=> />.
+transitivity{1} {
+    z <@ PBool.Sample.sample(size_out);
+  }
+  (true ==> ={z})
+  (true ==> z{1} = l{2})=>/>.
++ by inline*; auto.
+transitivity{1} {
+    z <@ LoopSnoc.sample(size_out);
+  }
+  (true ==> ={z})
+  (true ==> z{1} = l{2})=>/>; last first.
++ inline*; auto; sim.
+  by while(={l, i} /\ n{1} = size_out); auto; smt(cats1).
+by call(Sample_LoopSnoc_eq); auto.
+qed.
+
+
+local equiv eq_IRO_RFWhile :
+  BIRO.IRO.f ~ RFWhile.get :
+  arg{1} = (x{2}, size_out) /\ inv BIRO.IRO.mp{1} RFList.m{2}
+  ==>
+  res{2} = of_list res{1} /\ size res{1} = size_out /\ inv BIRO.IRO.mp{1} RFList.m{2}.
+proof.
+proc; inline*; sp.
+rcondt{1} 1; 1: by auto.
+if{2}; sp; last first.
++ alias{1} 1 mp = BIRO.IRO.mp.
+  conseq(:_==> BIRO.IRO.mp{1} = mp{1} /\ size bs{1} = i{1} /\ i{1} = size_out /\
+        inv mp{1} RFList.m{2} /\
+        bs{1} = take i{1} (to_list (oget RFList.m{2}.[x{1}])))=> />.
+  - move=> &l &r 11?.
+    rewrite take_oversize 1:spec_dout 1:H4 //.
+    rewrite eq_sym to_listK => ->.
+    by have:=H3; rewrite domE; smt().
+  - smt(take_oversize spec_dout).
+  while{1}(BIRO.IRO.mp{1} = mp{1} /\ size bs{1} = i{1} /\ 
+        0 <= i{1} <= size_out /\ n{1} = size_out /\
+        inv mp{1} RFList.m{2} /\ x{1} \in RFList.m{2} /\
+        bs{1} = take i{1} (to_list (oget RFList.m{2}.[x{1}])))(size_out - i{1});
+      auto=> />.
+  + sp; rcondf 1; auto=> />; 1: smt().
+    move=> &h 8?.
+    rewrite size_rcons //=; do!split; 1, 2, 4: smt(size_ge0).
+    rewrite (take_nth witness) 1:spec_dout 1:size_ge0//=. 
+    rewrite - H6; congr; rewrite H4=> //=.
+    by apply H3=> //=.
+  smt(size_out_gt0 size_ge0 take0).
+auto=> //=.
+conseq(:_==> l{2} = bs{1} /\ size bs{1} = i{1} /\ i{1} = n{1} /\ n{1} = size_out /\
+  inv BIRO.IRO.mp{1} RFList.m{2}.[x{2} <- oget (of_list l{2})])=> />. 
++ smt(get_setE spec2_dout).
++ smt(get_setE spec2_dout).
+alias{1} 1 m = BIRO.IRO.mp; sp.
+conseq(:_==> l{2} = bs{1} /\ size bs{1} = i{1} /\ i{1} = n{1} /\ 
+  n{1} = size_out /\ inv m{1} RFList.m{2} /\
+  (forall j, (x{1}, j) \in BIRO.IRO.mp{1} => 0 <= j < i{1}) /\
+  (forall l j, l <> x{1} => m{1}.[(l,j)] = BIRO.IRO.mp{1}.[(l,j)]) /\
+  (forall j, 0 <= j < i{1} => (x{1}, j) \in BIRO.IRO.mp{1}) /\
+  (forall j, 0 <= j < i{1} => BIRO.IRO.mp{1}.[(x{1},j)] = Some (nth witness bs{1} j))).
++ move=> /> &l &r 11?; do!split; ..-2 : smt(domE mem_set).
+  move=> l j Hin.
+  rewrite get_setE/=.
+  case: (l = x{r}) => [<<-|].
+  - rewrite oget_some H8; 1:smt(); congr; congr.
+    by rewrite eq_sym to_listK; smt(spec2_dout).
+  move=> Hneq.
+  by rewrite -(H6 _ _ Hneq) H2; smt(domE).
+while(l{2} = bs{1} /\ size bs{1} = i{1} /\ 0 <= i{1} <= n{1} /\ ={i} /\
+  n{1} = size_out /\ inv m{1} RFList.m{2} /\
+  (forall j, (x{1}, j) \in BIRO.IRO.mp{1} => 0 <= j < i{1}) /\
+  (forall l j, l <> x{1} => m{1}.[(l,j)] = BIRO.IRO.mp{1}.[(l,j)]) /\
+  (forall j, 0 <= j < i{1} => (x{1}, j) \in BIRO.IRO.mp{1}) /\
+  (forall j, 0 <= j < i{1} => BIRO.IRO.mp{1}.[(x{1},j)] = Some (nth witness bs{1} j))).
++ sp; rcondt{1} 1; auto=> />.
+  - smt().
+  move=> &l &r 13?.
+  rewrite get_setE/=oget_some/=size_rcons/=; do!split; 1,2: smt(size_ge0).
+  - smt(mem_set).
+  - smt(get_setE).
+  - smt(mem_set).
+  - move=>j Hj0 Hjsize; rewrite get_setE/=nth_rcons.
+    case: (j = size bs{l})=>[->>//=|h].
+    have/=Hjs:j < size bs{l} by smt().
+    by rewrite Hjs/=H8//=.
+by auto; smt(size_out_gt0).
+qed.
+
+
+local module ExtendSample (F : OFUNCTIONALITY) = {
+  proc init = F.init
+  proc f (x : bool list, k : int) = {
+    var y;
+    if (k <= size_out) {
+      y <@ F.f(x,size_out);
+      y <- omap (take k) y;
+    } else {
+      y <@ F.f(x,k);
+    }
+    return y;
+  }
+}.
+
+
+local equiv eq_extend :
+  ExtendSample(FSome(BIRO.IRO)).f ~ ExtendOutputSize(FSetSize(FSome(BIRO.IRO))).f :
+  ={arg} /\ eq_extend_size BIRO.IRO.mp{1} BIRO.IRO.mp{2} Log.m{2} ==>
+  ={res} /\ eq_extend_size BIRO.IRO.mp{1} BIRO.IRO.mp{2} Log.m{2}.
+proof.
+proc; inline*; auto; sp.
+rcondt{2} 1; 1: auto.
+if{1}; sp.
+- rcondt{1} 1; auto.
+  rcondf{2} 8; 1: auto.
+  - conseq(:_==> true); 1: smt(). 
+    by while(true); auto.
+  auto=> /=.
+  conseq(:_==> ={bs, k} /\ size bs{1} = size_out /\
+    eq_extend_size BIRO.IRO.mp{1} BIRO.IRO.mp{2} Log.m{2})=> //=.
+  - smt(cats0 to_listK spec2_dout).
+  while(={k, bs, n, x2} /\ i{1} = i0{2} /\ n{1} = size_out /\
+      0 <= i{1} <= n{1} /\ size bs{1} = i{1} /\
+      eq_extend_size BIRO.IRO.mp{1} BIRO.IRO.mp{2} Log.m{2}).
+  - by sp; if; auto; smt(domE get_setE size_rcons).
+  by auto; smt(size_eq0 size_out_gt0).
+rcondt{1} 1; 1: auto.
+splitwhile{1} 1 : i0 < size_out; auto=> /=.
+while( (i0, n0, x3){1} = (i, k, x){2} /\ bs0{1} = prefix{2} ++ suffix{2} /\
+    size_out <= i{2} <= k{2} /\ eq_extend_size BIRO.IRO.mp{1} BIRO.IRO.mp{2} Log.m{2}).
++ by sp; if; auto; smt(domE get_setE size_out_gt0 rcons_cat).
+auto=> //=.
+conseq(:_==> ={i0} /\ size bs{2} = i0{1} /\ (i0, x3){1} = (n, x2){2} /\
+    bs0{1} = bs{2} /\ size bs{2} = size_out /\
+    eq_extend_size BIRO.IRO.mp{1} BIRO.IRO.mp{2} Log.m{2}). 
++ smt(cats0 take_oversize spec_dout to_listK spec2_dout).
+while(={i0} /\ x3{1} = x2{2} /\ 0 <= i0{1} <= n{2} /\ n{2} = size_out /\
+    bs0{1} = bs{2} /\ size bs{2} = i0{1} /\ size_out <= n0{1} /\
+    eq_extend_size BIRO.IRO.mp{1} BIRO.IRO.mp{2} Log.m{2}).
++ by sp; if; auto; smt(size_rcons domE get_setE size_rcons mem_set).
+by auto; smt(size_out_gt0).
+qed.
+
+
+local lemma of_listK l : of_list (to_list l) = Some l.
+proof.
+by rewrite -to_listK.
+qed.
+
+local module Fill_In (F : RO) = {
+  proc init = F.init
+  proc f (x : bool list, n : int) = {
+    var l, b, i;
+    i <- 0;
+    l <- [];
+    while (i < n) {
+      b <@ F.get((x,i));
+      l <- rcons l b;
+      i <- i + 1;
+    }
+    while (i < size_out) {
+      F.sample((x,i));
+      i <- i + 1;
+    }
+    return l;
+  }
+}.
+
+print module RO.
+
+local equiv eq_eager_ideal :
+  BIRO.IRO.f ~ Fill_In(LRO).f :
+  ={arg} /\ BIRO.IRO.mp{1} = RO.m{2} ==>
+  ={res} /\ BIRO.IRO.mp{1} = RO.m{2}.
+proof.
+proc; inline*; sp; rcondt{1} 1; auto.
+while{2}(bs{1} = l{2} /\ BIRO.IRO.mp{1} = RO.m{2})(size_out - i{2}).
++ by auto=> />; smt().
+conseq(:_==> bs{1} = l{2} /\ BIRO.IRO.mp{1} = RO.m{2}); 1: smt().
+while(={i, n, x} /\ bs{1} = l{2} /\ BIRO.IRO.mp{1} = RO.m{2}).
++ sp; if{1}.
+  - by rcondt{2} 2; auto=> />.
+  by rcondf{2} 2; auto=> />; smt(dbool_ll).
+by auto.
+qed.
+
+local equiv eq_eager_ideal2 :
+  ExtendSample(FSome(BIRO.IRO)).f ~ FSome(Fill_In(RO)).f :
+  ={arg} /\ BIRO.IRO.mp{1} = RO.m{2} ==>
+  ={res} /\ BIRO.IRO.mp{1} = RO.m{2}.
+proof.
+proc; inline*; sp.
+if{1}; sp.
++ rcondt{1} 1; auto=> /=/>.
+  conseq(:_==> take k{1} bs{1} = l{2} /\ BIRO.IRO.mp{1} = RO.m{2}).
+  * smt().
+  case: (0 <= n{2}); last first.
+  + rcondf{2} 1; 1: by auto; smt(). 
+    conseq(:_==> BIRO.IRO.mp{1} = RO.m{2} /\ ={i} /\ n{1} = size_out /\ x2{1} = x0{2})=> />.
+    - smt(take_le0).
+    while(={i} /\ x2{1} = x0{2} /\ n{1} = size_out /\ BIRO.IRO.mp{1} = RO.m{2}).
+    - sp; if{1}.
+      - by rcondt{2} 2; auto=> />.
+      by rcondf{2} 2; auto=> />; smt(dbool_ll).
+    by auto=> />.
+  splitwhile{1} 1 : i < k.
+  while(={i} /\ n{1} = size_out /\ x2{1} = x0{2} /\  BIRO.IRO.mp{1} = RO.m{2} /\
+      take k{1} bs{1} = l{2} /\ size bs{1} = i{1} /\ k{1} <= i{1} <= size_out).
+  * sp; if{1}.
+    - by rcondt{2} 2; auto; smt(dbool_ll cats1 take_cat cats0 take_size size_rcons).
+    by rcondf{2} 2; auto; smt(dbool_ll cats1 take_cat cats0 take_size size_rcons).
+  conseq(:_==> ={i} /\ n{1} = size_out /\ x2{1} = x0{2} /\  BIRO.IRO.mp{1} = RO.m{2} /\
+      bs{1} = l{2} /\ size bs{1} = i{1} /\ k{1} = i{1}).
+  + smt(take_size).
+  while(={i} /\ x2{1} = x0{2} /\ n{1} = size_out /\ k{1} = n{2} /\
+      0 <= i{1} <= k{1} <= size_out /\ bs{1} = l{2} /\ size bs{1} = i{1} /\
+      BIRO.IRO.mp{1} = RO.m{2}).
+  + sp; if{1}.
+    - by rcondt{2} 2; auto; smt(size_rcons).
+    by rcondf{2} 2; auto; smt(size_rcons dbool_ll).
+  by auto; smt(size_ge0 size_out_gt0).
+rcondt{1} 1; auto.
+rcondf{2} 2; 1: auto.
++ conseq(:_==> i = n); 1: smt().
+  by while(i <= n); auto=> />; smt(size_out_gt0).
+while(i0{1} = i{2} /\ x3{1} = x0{2} /\ n0{1} = n{2} /\ bs0{1} = l{2} /\ 
+    BIRO.IRO.mp{1} = RO.m{2}).
++ sp; if{1}.
+  - by rcondt{2} 2; auto=> />.
+  by rcondf{2} 2; auto; smt(dbool_ll).
+by auto=> />.
+qed.
+
+local module Dist (F : RO) = {
+  proc distinguish = SHA3_OIndiff.OIndif.OIndif(FSome(Fill_In(F)),
+      OSimulator(FSome(Fill_In(F))), ODRestr(Dist_of_P2Adv(A))).main
+}.
+
+local module Game (F : RO) = {
+  proc distinguish () = {
+    var bo;
+    OSimulator(FSome(Fill_In(F))).init();
+    Counter.c <- 0;
+    Log.m <- empty;
+    F.init();
+    bo <@ Dist(F).distinguish();
+    return bo;
+  }
+}.
+
+local lemma eager_ideal &m :
+    Pr[SHA3_OIndiff.OIndif.OIndif(FSome(BIRO.IRO),
+      OSimulator(FSome(BIRO.IRO)),
+      ODRestr(Dist_of_P2Adv(A))).main() @ &m : res] =
+    Pr[SHA3_OIndiff.OIndif.OIndif(ExtendSample(FSome(BIRO.IRO)),
+      OSimulator(ExtendSample(FSome(BIRO.IRO))),
+      ODRestr(Dist_of_P2Adv(A))).main() @ &m : res].
+proof.
+cut->: 
+  Pr[SHA3_OIndiff.OIndif.OIndif(FSome(BIRO.IRO),
+    OSimulator(FSome(BIRO.IRO)),
+    ODRestr(Dist_of_P2Adv(A))).main() @ &m : res] =
+  Pr[Game(LRO).distinguish() @ &m : res].
++ byequiv=> //=; proc.
+  inline{2} 1; sp; inline{2} 1; sp; inline{2} 1; sp; inline{2} 1; sp.
+  inline{1} 1; inline{2} 1; sp.
+  inline{1} 1; inline{2} 1; sp.
+  inline{1} 1; inline{2} 1; sp.
+  inline{1} 1; inline{2} 1; sp.
+  inline{1} 1; inline{2} 1; sp.
+  inline{1} 1; inline{2} 1; sp; sim.
+  seq 1 1 : (={m', glob Dist_of_P2Adv, glob OFC} /\ BIRO.IRO.mp{1} = RO.m{2}); last first.
+  - inline{1} 1; inline{2} 1; sp; sim.
+    inline{1} 1; inline{2} 1; sp; sim; if; auto.
+    * inline{1} 1; inline{2} 1; sp; sim.
+      inline{1} 7; inline{2} 7; sim.
+      inline{1} 8; inline{2} 8; sim.
+      swap 3 -2; sp.
+      case: (increase_counter Counter.c{1} m'{1} size_out <= SHA3Indiff.limit). 
+      + rcondt{1} 10; 1: auto.
+        - inline*; auto.
+          by sp; rcondt 1; auto; conseq(:_==> true); auto.
+        rcondt{2} 10; 1: auto.
+        - inline*; auto.
+          by conseq(:_==> true); auto.
+        sim.
+        inline{1} 10; inline{2} 10; sim.
+        call eq_eager_ideal; auto.
+        by call eq_eager_ideal; auto.
+      rcondf{1} 10; 1: auto.
+      - inline*; auto.
+        by sp; rcondt 1; auto; conseq(:_==> true); auto.
+      rcondf{2} 10; 1: auto.
+      - inline*; auto.
+        by conseq(:_==> true); auto.
+      by auto; call eq_eager_ideal; auto.
+    sp; inline{1} 1; inline{2} 1; sp; sim.
+    inline{1} 1; inline{2} 1; sp; sim.
+    if; auto.
+    inline{1} 1; inline{2} 1; sp; sim.
+    by auto; call eq_eager_ideal; auto.
+  call(: ={glob OFC, glob OSimulator, glob Dist_of_P2Adv} /\ 
+      BIRO.IRO.mp{1} = RO.m{2}); auto.
+  - proc; sp; if; auto.
+    inline{1} 1; inline{2} 1; sp; sim; if; 1: auto; sim.
+    if; 1: auto; sim; sp.
+    if; 1: auto; 1: smt(); sim.
+    * inline{1} 1; inline{2} 1; sp; sim.
+      by call eq_eager_ideal; auto; smt().
+    smt().
+  - by proc; inline*; sim.
+  proc; sim.
+  inline{1} 1; inline{2} 1; sp; sim; if; 1: auto; sim.
+  inline{1} 1; inline{2} 1; sp; sim.
+  by call eq_eager_ideal; auto.
+cut->: 
+  Pr[SHA3_OIndiff.OIndif.OIndif(ExtendSample(FSome(BIRO.IRO)),
+    OSimulator(ExtendSample(FSome(BIRO.IRO))),
+    ODRestr(Dist_of_P2Adv(A))).main() @ &m : res] =
+  Pr[Game(RO).distinguish() @ &m : res].
++ byequiv=> //=; proc.
+  inline{2} 1; sp; inline{2} 1; sp; inline{2} 1; sp; inline{2} 1; sp.
+  inline{1} 1; inline{2} 1; sp.
+  inline{1} 1; inline{2} 1; sp.
+  inline{1} 1; inline{2} 1; sp.
+  inline{1} 1; inline{2} 1; sp.
+  inline{1} 1; inline{2} 1; sp.
+  inline{1} 1; inline{2} 1; sp; sim.
+  seq 1 1 : (={m', glob Dist_of_P2Adv, glob OFC} /\ BIRO.IRO.mp{1} = RO.m{2}); last first.
+  - inline{1} 1; inline{2} 1; sp; sim.
+    inline{1} 1; inline{2} 1; sp; sim; if; auto.
+    * inline{1} 6; inline{2} 6; sim.
+      inline{1} 7; inline{2} 7; sim.
+      swap 2 -1; sp.
+      case: (increase_counter Counter.c{1} m'{1} size_out <= SHA3Indiff.limit). 
+      + rcondt{1} 9; 1: auto.
+        - inline*; auto.
+          by sp; rcondt 1; auto; conseq(:_==> true); auto.
+        rcondt{2} 9; 1: auto.
+        - inline*; auto.
+          by conseq(:_==> true); auto.
+        sim.
+        call eq_eager_ideal2; auto.
+        by call eq_eager_ideal2; auto.
+      rcondf{1} 9; 1: auto.
+      - inline*; auto.
+        by sp; rcondt 1; auto; conseq(:_==> true); auto.
+      rcondf{2} 9; 1: auto.
+      - inline*; auto.
+        by conseq(:_==> true); auto.
+      by auto; call eq_eager_ideal2; auto.
+    sp; inline{1} 1; inline{2} 1; sp; sim.
+    inline{1} 1; inline{2} 1; sp; sim.
+    if; auto.
+    by auto; call eq_eager_ideal2; auto.
+  call(: ={glob OFC, glob OSimulator, glob Dist_of_P2Adv} /\ 
+      BIRO.IRO.mp{1} = RO.m{2}); auto.
+  - proc; sp; if; auto.
+    inline{1} 1; inline{2} 1; sp; sim; if; 1: auto; sim.
+    if; 1: auto; sim; sp.
+    if; 1: auto; 1: smt(); sim.
+    * by call eq_eager_ideal2; auto; smt().
+    smt().
+  - by proc; inline*; sim.
+  proc; sim.
+  inline{1} 1; inline{2} 1; sp; sim; if; 1: auto; sim.
+  by call eq_eager_ideal2; auto.
+rewrite eq_sym; byequiv=> //=; proc. 
+by call(RO_LRO_D Dist); inline*; auto=> />.
+qed.
+
+
+
+
+local lemma rw_ideal_2 &m (mess : bool list):
+    Dist_of_P2Adv.m{m} = mess =>
+    Pr[SHA3_OIndiff.OIndif.OIndif(FSome(BIRO.IRO), OSimulator(FSome(BIRO.IRO)), 
+      ODRestr(Dist_of_P2Adv(A))).main() @ &m : res] <=
+    Pr[SORO.SecondPreimage(SORO_P2(A), RFList).main(mess) @ &m : res].
+proof.
+move=> Heq.
+have->:Pr[SORO.SecondPreimage(SORO_P2(A), RFList).main(mess) @ &m : res] =
+       Pr[SORO.SecondPreimage(SORO_P2(A), RFWhile).main(mess) @ &m : res].
++ byequiv(: ={glob A, arg} /\ arg{1} = mess ==> _)=>//=; proc.
+  inline{1} 1; inline{2} 1; sp.
+  inline{1} 1; inline{2} 1; sp.
+  inline{1} 1; inline{2} 1; sp.
+  inline{1} 1; inline{2} 1; sp.
+  inline{1} 1; inline{2} 1; sp.
+  seq 1 1 : (={mi, m1, glob A, glob SORO.Bounder, glob RFList, glob Dist_of_P2Adv}); last first.
+  - sp; inline{1} 2; inline{2} 2; inline{1} 1; inline{2} 1; sp; sim.
+    if; auto.
+    - sp; case: (SORO.Bounder.bounder{1} < sigma).
+      * rcondt{1} 5; 1: auto.
+        + by inline*; auto; conseq(:_==> true); auto.
+        rcondt{2} 5; 1: auto.
+        + by inline*; auto; conseq(:_==> true); auto.
+        call(rw_RF_List_While); auto.
+        by call(rw_RF_List_While); auto=> />.
+      rcondf{1} 5; 1: auto.
+      + by inline*; auto; conseq(:_==> true); auto.
+      rcondf{2} 5; 1: auto.
+      + by inline*; auto; conseq(:_==> true); auto.
+      by auto; call(rw_RF_List_While); auto.
+    by sp; if; auto; call(rw_RF_List_While); auto.
+  call(: ={glob SORO.Bounder, glob RFList, glob OSimulator, glob OPC, glob Log,
+         glob Dist_of_P2Adv}); auto.
+  - proc; sp; if; auto.
+    inline{1} 1; inline{2} 1; sp; if; 1, 3: auto; sim.
+    if; 1: auto; sim; sp; sim; if; auto=> />; 1: smt(); sim.
+    + inline{1} 1; inline{2} 1; sp; sim.
+      inline{1} 1; inline{2} 1; sp; if; auto=> />.
+      - by call(rw_RF_List_While); auto; smt(). 
+      smt().
+    smt().
+  - by sim. 
+  proc; sim; inline{1} 1; inline{2} 1; sp; if; auto.
+  inline{1} 1; inline{2} 1; sp; sim.
+  inline{1} 1; inline{2} 1; sp; if; auto; sim.
+  by call(rw_RF_List_While); auto.
+rewrite (eager_ideal &m).
+have->:Pr[SHA3_OIndiff.OIndif.OIndif(ExtendSample(FSome(BIRO.IRO)),
+         OSimulator(ExtendSample(FSome(BIRO.IRO))),
+          ODRestr(Dist_of_P2Adv(A))).main() @ &m : res] =
+       Pr[SHA3_OIndiff.OIndif.OIndif(ExtendSample(FSome(BIRO.IRO)),
+         OSimulator(ExtendOutputSize(FSetSize(FSome(BIRO.IRO)))),
+         ODRestr(Dist_of_P2Adv(A))).main() @ &m : res].
++ byequiv=> //=; proc; inline*; sp.
+  (* TODO : refaire un seq de + pour gérer mieux les 2 boucles, ou faire un lemme général *)
+
+
+  seq 1 1 : (={m', glob OSimulator, glob OFC, glob Dist_of_P2Adv} /\
+         eq_extend_size BIRO.IRO.mp{1} BIRO.IRO.mp{2} Log.m{2}); last first.
+  - sp; if; auto; sp; if; auto; sp; rcondt{1}1; 1: auto. 
+    * rcondt{2} 1; 1: auto.
+  
+      while(={i, n, bs, x3} /\ size bs{1} = i{1} /\
+           eq_extend_size BIRO.IRO.mp{1} BIRO.IRO.mp{2} Log.m{2} /\
+           n{1} = size_out /\ 0 <= i{1} <= n{1}); auto.
+      * by sp; if; auto; smt(domE get_setE size_rcons).
+      smt(size_out_gt0 take_oversize size_out_gt0).
+    * by auto; rcondf{1} 1; auto.
+    * rcondt{2} 1; 1: auto; move=> />; auto.
+      by while(={i0, n0}); auto; sp; if{1}; if{2}; auto; smt(dbool_ll).
+  call(: ={glob OSimulator, glob OFC} /\
+         eq_extend_size BIRO.IRO.mp{1} BIRO.IRO.mp{2} Log.m{2}); last first; auto.
+  + smt(mem_empty).
+  + proc; sp; if; auto. 
+    inline{1} 1; inline{2} 1; sp; if; 1, 3: auto.
+    if; 1, 3: auto; sp.
+    if; 1: auto; 1: smt(); last first.
+    - by conseq=> />; sim; smt().
+    wp=> />; 1: smt().
+    rnd; auto=> />; 1: smt().
+    call(eq_extend); last by auto; smt().
+  + by proc; sp; if; auto; inline{1} 1; inline{2} 1; sp; if; auto.
+  proc; sp; inline{1} 1; inline{2} 1; sp; if; auto.
+  inline*; sp.
+  rcondt{1} 1; 1: auto; rcondt{2} 1; 1: auto; sp.
+  rcondt{1} 1; 1: auto; rcondt{2} 1; 1: auto; sp; auto.
+  conseq(:_==> ={bs} /\ eq_extend_size BIRO.IRO.mp{1} BIRO.IRO.mp{2} Log.m{2}); 
+    1: by auto.
+  while(={i, n, x3, bs} /\ 0 <= i{1} <= size_out /\ n{1} = size_out /\ 
+      eq_extend_size BIRO.IRO.mp{1} BIRO.IRO.mp{2} Log.m{2}).
+  - by sp; if; auto; smt(domE get_setE size_rcons).
+  by auto; smt(size_out_gt0).
+byequiv=> //=; proc.
+inline{1} 1; inline{2} 2; sp.
+inline{1} 1; inline{2} 3; swap{2}[1..2]1; sp.
+inline{1} 1; inline{2} 3; sp.
+inline{1} 1; sp.
+inline{1} 1; sp.
+swap{2} 1 1; sp; swap{2}[1..2]3; sp.
+inline{1} 1; sp; auto. 
+seq 2 5 : (={glob A, glob OSimulator, glob Counter, glob Log, hash, m} /\
+         inv BIRO.IRO.mp{1} RFList.m{2} /\
+         SORO.Bounder.bounder{2} <= Counter.c{1}); last first.
++ inline{1} 1; inline{2} 1; sp; inline{1} 1; sp; auto.
+  if{1}; sp; last first.
+  - conseq(:_==> true)=> />.
+    inline*; if{2}; auto; sp; if{2}; auto.
+    by while{2}(true)(size_out - i{2}); auto=>/>; smt(dbool_ll).
+  rcondt{2} 1; 1: by auto=> />; smt(divz_ge0 gt0_r size_ge0).
+  inline{1} 1; sp; auto.
+  rcondt{1} 1; auto=> /=. 
+  inline{1} 1; sp; auto.
+  by call(eq_IRO_RFWhile); auto; smt(take_oversize).
+auto; call(: ={glob OSimulator, glob Counter, glob Log} /\ 
+    inv BIRO.IRO.mp{1} RFList.m{2} /\
+    SORO.Bounder.bounder{2} <= Counter.c{1}); auto; last first.
++ by inline*; auto; smt(mem_empty).
++ proc; sp; if; auto=> />; 1: smt(). 
+  inline{1} 1; inline{2} 1; sp; auto.
+  if; 1, 3: auto; -1: smt().
+  if; 1, 3: auto; -1: smt().
+  sp; if; 1: auto; 1: smt(); last first.
+  - by conseq(:_==> ={y, glob OSimulator}); 1: smt(); sim; smt().
+  inline{1} 1; inline{2} 1; sp.
+  inline{1} 1; inline{2} 1; sp.
+  rcondt{2} 1; 1: by auto; smt().
+  sp.
+  seq 3 2 : (={x0, x1, o1, k0, Log.m, suffix, glob OSimulator} /\
+      inv BIRO.IRO.mp{1} RFList.m{2} /\ 
+      SORO.Bounder.bounder{2} <= Counter.c{2} + 1); last first.
+  - by conseq(:_==> ={y, x1, glob OSimulator, Log.m}); 1: smt(); sim=> />.
+  inline{1} 1; auto.
+  by call(eq_IRO_RFWhile); auto; smt().
++ by proc; inline*; sp; if; auto; sp; if; auto=> />; smt().
+proc.
+inline{1} 1; inline{2} 1; sp; if; auto=> /=.
+inline{1} 1; inline{2} 1; sp.
+rcondt{1} 1; 1: auto.
+inline{1} 1; auto.
+rcondf{2} 4; 1: auto. 
++ inline*; auto; sp; if; auto; sp; if; auto=> />; conseq(:_==> true); 1: smt().
+  by while(true); auto.
+inline{2} 1; sp.
+rcondt{2} 1; 1: by auto; smt(divz_ge0 gt0_r size_ge0).
+auto; call eq_IRO_RFWhile; auto=> />.
+move=> &l &r 13?; split; 2: smt(divz_ge0 gt0_r size_ge0).
+rewrite 2!oget_some cats0 take_oversize 1:/# take_oversize 1:spec_dout //=.
+have h:=spec2_dout result_L H5.
+have-> := some_oget _ h.
+by rewrite eq_sym -to_listK; congr.
+qed.
+
+local lemma rw_ideal &m:
+    Pr[SHA3_OIndiff.OIndif.OIndif(FSome(BIRO.IRO), OSimulator(FSome(BIRO.IRO)), 
+      ODRestr(Dist_of_P1Adv(A))).main() @ &m : res] <=
+    Pr[SORO.SecondPreimage(SORO_P1(A),RF(SORO.RO.RO)).main() @ &m : res].
+proof.
+rewrite (StdOrder.RealOrder.ler_trans _ _ _ (rw_ideal_2 &m)).
+byequiv(: ={glob A} ==> _) => //=; proc; inline*; sp; wp.
+swap{2} 2; sp; swap{2}[1..2] 6; sp.
+swap{1} 2; sp; swap{1}[1..2] 6; sp.
+seq 2 2 : (
+  Log.m{1} = empty /\
+  SHA3Indiff.Simulator.m{1} = empty /\
+  SHA3Indiff.Simulator.mi{1} = empty /\
+  SHA3Indiff.Simulator.paths{1} = empty.[c0 <- ([], b0)] /\
+  Gconcl_list.BIRO2.IRO.mp{1} = empty /\
+  SORO.Bounder.bounder{1} = 0 /\
+  RFList.m{1} = empty /\
+  Counter.c{2} = 0 /\
+  ={Log.m, glob SHA3Indiff.Simulator, glob SORO.Bounder, glob Counter} /\
+  SORO.RO.RO.m{2} = empty /\ ={glob A, h, hash}); 1: auto=> />. 
+seq 1 1 : (={glob A, glob SHA3Indiff.Simulator, glob SORO.Bounder, glob Counter, 
+    glob Log, mi, h, hash} /\ RFList.m{1} = SORO.RO.RO.m{2}).
++ call(: ={glob SHA3Indiff.Simulator, glob SORO.Bounder, glob Counter, glob Log} /\ 
+    RFList.m{1} = SORO.RO.RO.m{2}); auto.
+  - proc; sp; if; 1, 3: auto; sp.
+    inline *; sp; sim.
+    if; 1: auto; sim. 
+    if; 1: auto; sim.
+    sp; if; 1: (auto; smt()); sim; 2: smt(). 
+    sp; if; 1: auto; sim; -1: smt().
+    sp; if{1}.
+    * rcondt{2} 2; auto; 1: smt(BlockSponge.parse_valid).
+      rnd (fun l => oget (of_list l)) to_list; auto=> />.
+      move=> &l &r 10?; split; 1: smt(of_listK).
+      rewrite -dout_equal_dlist=> ?; split=> ?.
+      + by rewrite dmapE=> h{h}; apply mu_eq=> x; smt(to_list_inj).
+      move=> sample.
+      rewrite !get_setE/=oget_some/=dout_full/= => h; split; 2: smt(). 
+      rewrite eq_sym to_listK; apply some_oget.
+      apply spec2_dout.
+      by move:h; rewrite supp_dmap; smt(spec_dout).
+    by auto; smt(dout_ll).
+  - by proc; inline*; sp; if; auto; sp; if; auto.
+  - proc; inline*; sp; if; auto; sp; if; auto; sp; sim.
+    if{1}.
+    * rcondt{2} 2; auto.
+      rnd (fun l => oget (of_list l)) to_list; auto=> />.
+      move=> &l 4?; split=> ?; 1: smt(of_listK).
+      rewrite -dout_equal_dlist; split=> ?.
+      * by rewrite dmapE=> h{h}; apply mu_eq=> x; smt(to_list_inj).
+      move=> sample.
+      rewrite supp_dmap dout_full/= =>/> a.
+      by rewrite get_setE/=oget_some/= dout_full/=; congr; rewrite of_listK oget_some.
+  by auto; smt(dout_ll).
+sp; if; 1, 3: auto; sp; wp 1 2.
+if{1}.
++ wp=> />.
+  rnd (fun x => oget (of_list x)) to_list; auto=> />.
+  move=> &l c Hc Hnin; split.
+  - move=> ret Hret. search to_list. 
+    by have/= ->:= (to_listK ret (to_list ret)).
+  move=> h{h}; split.
+  - move=> ret Hret; rewrite -dout_equal_dlist.
+    rewrite dmapE /=; apply mu_eq=> //= x /=.
+    by rewrite /(\o) /pred1/=; smt(to_list_inj).
+  move=> h{h} l Hl. 
+  rewrite dout_full /=.
+  have:= spec2_dout l.
+  have:=supp_dlist dbool size_out l _; 1: smt(size_out_gt0).
+  rewrite Hl/==> [#] -> h{h} /= H.
+  have H1:=some_oget _ H.
+  have:=to_listK (oget (of_list l)) l; rewrite {2}H1/= => -> /= {H H1}.
+  by rewrite get_setE/=.
+by auto=> />; smt(dout_ll).
+qed.
+
+
+local lemma leq_ideal &m :
+    Pr[SHA3_OIndiff.OIndif.OIndif(FSome(BIRO.IRO), OSimulator(FSome(BIRO.IRO)), 
+      ODRestr(Dist_of_P1Adv(A))).main() @ &m : res] <= (sigma + 1)%r / 2%r ^ size_out.
+proof.
+rewrite (StdOrder.RealOrder.ler_trans _ _ _ (rw_ideal &m)).
+rewrite (StdOrder.RealOrder.ler_trans _ _ _ (RO_is_preimage_resistant (SORO_P1(A)) &m)).
+by rewrite doutE1.
+qed.
+
+
+
+  local lemma rw_real &m : 
+      Pr[SecondPreimage(A, OSponge, PSome(Perm)).main() @ &m : res] =
+      Pr[SHA3_OIndiff.OIndif.OIndif(FSome(Sponge(Poget(PSome(Perm)))), PSome(Perm), 
+        ODRestr(Dist_of_P1Adv(A))).main() @ &m : res].
   proof.
-  apply (Sponge_coll_resistant (AdvCollisionSHA3(A)) _ &m).
-  by move=> F F_ll; proc; inline*; call(A_ll (X(F))); auto; proc; call F_ll; auto.
+  byequiv=>//=; proc; inline*; sp; wp=> />.
+  swap{1} 4; sp. 
+  seq 2 2 : (={glob A, glob Perm, hash, m} /\ Bounder.bounder{1} = Counter.c{2}).
+  + call(: ={glob Perm} /\ Bounder.bounder{1} = Counter.c{2})=> //=.
+    - by proc; inline*; sp; if; auto; 2:sim=> />; 1: smt().
+    - by proc; inline*; sp; if; auto; 2:sim=> />; 1: smt().
+    - proc; inline*; sp; if; auto; sp=> />.
+      by conseq(:_==> ={z0, glob Perm})=> />; sim.
+    by auto. 
+  by sp; if; auto=>/=; sim; auto.
   qed.
 
+lemma Sponge_preimage_resistant &m:
+    (forall (F <: OIndif.ODFUNCTIONALITY) (P <: OIndif.ODPRIMITIVE),
+      islossless F.f => islossless P.f => islossless P.fi => islossless A(F,P).guess) =>
+    Pr[SecondPreimage(A, OSponge, PSome(Perm)).main() @ &m : res] <=
+    (limit ^ 2 - limit)%r / (2 ^ (r + c + 1))%r +
+    (4 * limit ^ 2)%r / (2 ^ c)%r +
+    (sigma + 1)%r / (2%r ^ size_out).
+proof.
+move=> A_ll.
+rewrite (rw_real &m).
+have := SHA3OIndiff (Dist_of_P1Adv(A)) &m _.
++ move=> F P Hp Hpi Hf; proc; inline*; sp; auto; call Hf; auto. 
+  call(A_ll (DFSetSize(F)) P _ Hp Hpi); auto.
+  - proc; inline*; auto; call Hf; auto.
+  smt(dout_ll).
+by have/#:=leq_ideal &m.
+qed.
 
-end section Collision.
+end section SecondSecondPreimage.
+
+
